Better support for pure functions in the axiomatic semantics.

assertions.v
@@ -6,7 +6,8 @@ statement, and [P] and [Q] are assertions called the pre and postcondition of
 if [P] holds for the state before execution of [s], and execution of [s]
 terminates, then [Q] will hold afterwards. Like (Appel/Blazy, 2007), we define
 assertions using a shallow embedding. That is, assertions are predicates over
-the contents of the stack and memory. *)
+the contents of the stack and memory. To support dealing with pure functions,
+assertions also range over environments of pure functions. *)
 
 (** This file defines the data type of assertions, the usual connectives of
 Hoare logic ([∧], [∨], [¬], [↔], [∀] and [∃]), the connectives of separation
@@ -18,32 +19,34 @@ Require Import SetoidList.
 Require Export expression_eval memory.
 
 (** * Definition of assertions *)
-(** We pack assertions into a record so we can register the projection
+(** We pack assertions into an inductive type so we can register the projection
 [assert_holds] as [Proper] for the setoid rewriting mechanism. *)
-Record assert := Assert {
-  assert_holds :> stack → mem → Prop
-}.
+Inductive assert := Assert: (purefuns → stack → mem → Prop) → assert.
+Definition assert_holds δ (P : assert) : stack → mem → Prop :=
+  let (P') := P in P' δ.
 
 Delimit Scope assert_scope with A.
 Bind Scope assert_scope with assert.
-Arguments assert_holds _%A _ _.
-Definition assert_as_Prop (P : assert) : Prop :=
-  ∀ ρ m, P ρ m.
-Coercion assert_as_Prop : assert >-> Sortclass.
+Arguments assert_holds _ _%A _ _.
 
-(** By defining a pre-order on assertions we automatically obtain the desired
-equality from the generic setoid equality on pre-orders. *)
-Instance assert_subseteq: SubsetEq assert := λ P Q,
-  ∀ ρ m, P ρ m → Q ρ m.
-Instance: PreOrder assert_subseteq.
-Proof.
-  split.
-  * by intros P ρ m.
-  * intros P1 P2 P3 H1 H2 ρ m ?. by apply H2, H1.
-Qed.
-Instance: Proper ((⊆) ==> (=) ==> (=) ==> impl) assert_holds.
+(** The relation [P ⊆@{δ} Q] states that the assertion [Q] is a logical
+consenquence of [P] in the environment of pure functions [δ]. The relation
+[P ≡@{δ} Q] states that [P] and [Q] are logically equivalent in the environment
+of pure functions [δ]. *)
+Instance assert_subseteq: SubsetEqEnv purefuns assert := λ δ P Q,
+  ∀ ρ m, assert_holds δ P ρ m → assert_holds δ Q ρ m.
+Instance assert_equiv: EquivEnv purefuns assert := λ δ P Q,
+  P ⊆@{δ} Q ∧ Q ⊆@{δ} P.
+Instance: PreOrder (assert_subseteq δ).
 Proof. firstorder. Qed.
-Instance: Proper ((≡) ==> (=) ==> (=) ==> iff) assert_holds.
+Instance: Equivalence (assert_equiv δ).
+Proof. firstorder. Qed.
+Instance: Proper ((≡@{δ}) ==> (≡@{δ}) ==> iff) (assert_subseteq δ).
+Proof. firstorder auto. Qed.
+
+Instance: Proper ((⊆@{δ}) ==> (=) ==> (=) ==> impl) (assert_holds δ).
+Proof. firstorder. Qed.
+Instance: Proper ((≡@{δ}) ==> (=) ==> (=) ==> iff) (assert_holds δ).
 Proof. firstorder. Qed.
 
 (** * Subclasses of assertions *)
@@ -53,25 +56,50 @@ Proof. firstorder. Qed.
   (Reynolds, 2002) these are called "pure".
 - [MemExt] collects assertions that are preserved under extensions of the
   memory. In (Reynolds, 2002) these are called "intuitionistic".
-- [UnlockIndep] collects assertions that are independent of unlocking the
-  memory.
+- [UnlockIndep] collects assertions that are independent of unlocking
+  sequenced locations in the memory.
+- [FunIndep fs] collections assertions that are independent of the denotations
+  of the pure functions [fs].
 
 This file contains instances of these type classes for the various connectives.
 We use instance resolution to automatically compose these instances to prove
 the above properties for composite assertions. *)
 Class StackIndep (P : assert) : Prop :=
-  stack_indep: ∀ ρ1 ρ2 m, P ρ1 m → P ρ2 m.
+  stack_indep: ∀ δ ρ1 ρ2 m, assert_holds δ P ρ1 m → assert_holds δ P ρ2 m.
 Class MemIndep (P : assert) : Prop :=
-  mem_indep: ∀ ρ m1 m2, P ρ m1 → P ρ m2.
+  mem_indep: ∀ δ ρ m1 m2, assert_holds δ P ρ m1 → assert_holds δ P ρ m2.
 Class MemExt (P : assert) : Prop :=
-  mem_ext: ∀ ρ m1 m2, P ρ m1 → m1 ⊆ m2 → P ρ m2.
+  mem_ext: ∀ δ ρ m1 m2,
+    assert_holds δ P ρ m1 → m1 ⊆ m2 → assert_holds δ P ρ m2.
 Class UnlockIndep (P : assert) : Prop :=
-  unlock_indep: ∀ Ω ρ m, P ρ m ↔ P ρ (mem_unlock Ω m).
+  unlock_indep: ∀ δ Ω ρ m,
+    assert_holds δ P ρ m ↔ assert_holds δ P ρ (mem_unlock Ω m).
+Class FunIndep (fs : funset) (P : assert) : Prop :=
+  fun_indep: ∀ δ1 δ2 ρ m,
+    (∀ f, f ∉ fs → δ1 !! f = δ2 !! f) →
+    assert_holds δ1 P ρ m ↔ assert_holds δ2 P ρ m.
 
 Instance mem_indep_ext P : MemIndep P → MemExt P.
 Proof. firstorder auto. Qed.
 Instance mem_indep_lock P : MemIndep P → UnlockIndep P.
 Proof. intros H. split; apply H. Qed.
+
+Lemma fun_indep_union_l P δ1 δ2 ρ m :
+  FunIndep (dom _ δ1) P →
+  assert_holds (δ1 ∪ δ2) P ρ m ↔ assert_holds δ2 P ρ m.
+Proof.
+  intros. apply fun_indep. intros f Hf. apply option_eq. intros F.
+  rewrite lookup_union_Some_raw. rewrite not_elem_of_dom in Hf.
+  intuition congruence.
+Qed.
+Lemma fun_indep_union_r P δ1 δ2 ρ m :
+  FunIndep (dom _ δ2) P →
+  assert_holds (δ1 ∪ δ2) P ρ m ↔ assert_holds δ1 P ρ m.
+Proof.
+  intros. apply fun_indep. intros f Hf. apply option_eq. intros F.
+  rewrite lookup_union_Some_raw. rewrite not_elem_of_dom in Hf.
+  intuition congruence.
+Qed.
 
 (** Invoke type class resolution when [auto] or [eauto] has to solve these
 constraints. *)
@@ -79,6 +107,7 @@ Hint Extern 100 (StackIndep _) => apply _.
 Hint Extern 100 (MemIndep _) => apply _.
 Hint Extern 100 (MemExt _) => apply _.
 Hint Extern 100 (UnlockIndep _) => apply _.
+Hint Extern 100 (FunIndep _ _) => apply _.
 
 (** Allow it to solve more complex assertions automatically. *)
 Hint Extern 1000 (MemIndep (match ?x with _ => _ end)) =>
@@ -89,70 +118,117 @@ Hint Extern 1000 (StackIndep (match ?x with _ => _ end)) =>
   destruct x : typeclass_instances.
 Hint Extern 1000 (UnlockIndep (match ?x with _ => _ end)) =>
   destruct x : typeclass_instances.
+Hint Extern 1000 (FunIndep _ (match ?x with _ => _ end)) =>
+  destruct x : typeclass_instances.
 
 (** * Tactics *)
 (** The tactic [solve_assert] will be used to automatically prove simple
 properties about assertions. It unfolds assertions using the unfold hint
 database [assert] and uses the [naive_solver] tactic to finish the proof. *)
 Hint Unfold
-  assert_as_Prop
-  StackIndep MemIndep MemExt UnlockIndep
-  equiv preorder_equiv subseteq subseteq assert_subseteq : assert.
+  StackIndep MemIndep MemExt UnlockIndep FunIndep assert_holds
+  equiv_env assert_equiv subseteq_env assert_subseteq : assert.
 
 (** In most situations we do not want [simpl] to unfold assertions and expose
 their internal definition. However, as the behavior of [simpl] cannot be
-changed locally using Ltac we block unfolding of [assert_holds] by [simpl]
-and define a custom tactic to perform this unfolding instead. Unfortunately,
-it does not work properly for occurrences of [assert_hold] under binders. *)
-Arguments assert_holds _ _ _ : simpl never.
+changed locally using Ltac we block unfolding of [assert_holds] by [simpl].
+Instead, to unfold assertions, we first unfold [assert_holds] everywhere,
+and then fold the projections back. This way of folding back is horrific,
+especialially the way of dealing with foldings under a fixed number of forall
+quantifiers. Since Ltac's support for dealing with open terms is limited, I
+am unaware how to do this better. *)
+Arguments assert_holds _ _ _ _ : simpl never.
 
-Tactic Notation "unfold_assert" "in" hyp(H) :=
-  repeat (progress (unfold assert_holds in H; simpl in H));
+Tactic Notation "fold_assert" "in" hyp(H) :=
   repeat match type of H with
-  | context C [let (x) := ?Q in x] =>
-    let X := context C [assert_holds Q] in change X in H
+  | context C [let (x) := ?Q in x ?δ] =>
+    let X := context C [assert_holds δ Q] in change X in H
+  | ∀ (x1 : ?A1) (x2 : ?A2) (x3 : ?A3), @?P' x1 x2 x3 =>
+    let H' := fresh in
+    let Q := fresh in evar (Q:A1 → A2 → A3 → Prop);
+    let Q' := eval unfold Q in Q in clear Q;
+    assert (∀ x1 x2 x3, P' x1 x2 x3 → Q' x1 x2 x3) as H' by
+     (intros ???; lazy beta;
+      progress repeat match goal with
+      | |- context C [let (x) := ?Q in x ?δ] =>
+        let X := context C [assert_holds δ Q] in change X
+    end; apply id);
+    specialize (λ x1 x2 x3, (H' x1 x2 x3) (H x1 x2 x3));
+    lazy beta in H'; clear H; rename H' into H
+  | ∀ (x1 : ?A1) (x2 : ?A2), @?P' x1 x2 =>
+    let H' := fresh in
+    let Q := fresh in evar (Q:A1 → A2 → Prop);
+    let Q' := eval unfold Q in Q in clear Q;
+    assert (∀ x1 x2, P' x1 x2 → Q' x1 x2) as H' by (intros ??; lazy beta;
+      progress repeat match goal with
+      | |- context C [let (x) := ?Q in x ?δ] =>
+        let X := context C [assert_holds δ Q] in change X
+    end; apply id);
+    specialize (λ x1 x2, (H' x1 x2) (H x1 x2));
+    lazy beta in H'; clear H; rename H' into H
+  | ∀ x1 : ?A1, @?P' x1 =>
+    let H' := fresh in
+    let Q := fresh in evar (Q:A1 → Prop);
+    let Q' := eval unfold Q in Q in clear Q;
+    assert (∀ x1, P' x1 → Q' x1) as H' by (intro; lazy beta;
+      progress repeat match goal with
+      | |- context C [let (x) := ?Q in x ?δ] =>
+        let X := context C [assert_holds δ Q] in change X
+    end; apply id);
+    specialize (λ x1, (H' x1) (H x1));
+    lazy beta in H'; clear H; rename H' into H
   end.
+Tactic Notation "fold_assert" :=
+  let rec go :=
+  lazymatch goal with
+  | |- ∀ x, _ => intro x; fold_assert in x; go; revert x
+  | |- ∀ _, _ => let H := fresh in intro H; fold_assert in H; go; revert H
+  | |- _ =>
+    repeat match goal with
+    | |- context C [let (x) := ?Q in x ?δ] =>
+    let X := context C [assert_holds δ Q] in change X
+    end
+  end in go.
+Tactic Notation "fold_assert" "in" "*" :=
+  fold_assert;
+  repeat match goal with H : _ |- _ => progress fold_assert in H end.
+
 Tactic Notation "unfold_assert" :=
-  repeat (progress (unfold assert_holds; simpl));
-  repeat match goal with
-  | |- context C [let (x) := ?Q in x] =>
-    let X := context C [assert_holds Q] in change X
-  end.
+  repeat (autounfold with assert; simpl);
+  fold_assert.
 Tactic Notation "unfold_assert" "in" "*" :=
-  unfold_assert;
-  repeat match goal with H : _ |- _ => progress unfold_assert in H end.
+  repeat (autounfold with assert in *; simpl in *);
+  fold_assert in *.
 
-(* Hint Extern 100 (_ ⊥ _) => solve_mem_disjoint : assert. *)
-
-Ltac solve_assert :=
+Tactic Notation "solve_assert" tactic3(tac) :=
   repeat intro;
   intuition;
-  repeat autounfold with assert in *;
   unfold_assert in *;
-  naive_solver (eauto with assert; congruence).
+  naive_solver tac.
+Tactic Notation "solve_assert" := solve_assert auto.
 
 (** * Hoare logic connectives *)
 (** Definitions and notations of the usual connectives of Hoare logic. *)
-Definition Prop_as_assert (P : Prop) : assert := Assert $ λ _ _, P.
+Definition Prop_as_assert (P : Prop) : assert := Assert $ λ _ _ _, P.
 Notation "⌜ P ⌝" := (Prop_as_assert P) (format "⌜  P  ⌝") : assert_scope.
 Notation "'True'" := (Prop_as_assert True) : assert_scope.
 Notation "'False'" := (Prop_as_assert False) : assert_scope.
 Definition assert_impl (P Q : assert) : assert :=
-  Assert $ λ ρ m, P ρ m → Q ρ m.
+  Assert $ λ δ ρ m, assert_holds δ P ρ m → assert_holds δ Q ρ m.
 Infix "→" := assert_impl : assert_scope.
 Notation "(→)" := assert_impl (only parsing) : assert_scope.
 Notation "( P →)" := (assert_impl P) (only parsing) : assert_scope.
 Notation "(→ Q )" := (λ P, assert_impl P Q) (only parsing) : assert_scope.
 
 Definition assert_and (P Q : assert) : assert :=
-  Assert $ λ ρ m, P ρ m ∧ Q ρ m.
+  Assert $ λ δ ρ m, assert_holds δ P ρ m ∧ assert_holds δ Q ρ m.
 Infix "∧" := assert_and : assert_scope.
 Notation "(∧)" := assert_and (only parsing) : assert_scope.
 Notation "( P ∧)" := (assert_and P) (only parsing) : assert_scope.
 Notation "(∧ Q )" := (λ P, assert_and P Q) (only parsing) : assert_scope.
 
 Definition assert_or (P Q : assert) : assert :=
-  Assert $ λ ρ m, P ρ m ∨ Q ρ m.
+  Assert $ λ δ ρ m, assert_holds δ P ρ m ∨ assert_holds δ Q ρ m.
 Infix "∨" := assert_or : assert_scope.
 Notation "(∨)" := assert_or (only parsing) : assert_scope.
 Notation "( P ∨)" := (assert_or P) (only parsing) : assert_scope.
@@ -164,57 +240,58 @@ Notation "(↔)" := assert_iff (only parsing) : assert_scope.
 Notation "( P ↔)" := (assert_iff P) (only parsing) : assert_scope.
 Notation "(↔ Q )" := (λ P, assert_iff P Q) (only parsing) : assert_scope.
 
-Definition assert_not (P : assert) : assert := Assert $ λ ρ m, ¬P ρ m.
+Definition assert_not (P : assert) : assert :=
+  Assert $ λ δ ρ m, ¬assert_holds δ P ρ m.
 Notation "¬ P" := (assert_not P) : assert_scope.
 
 Definition assert_forall {A} (P : A → assert) : assert :=
-  Assert $ λ ρ m, ∀ x, P x ρ m.
+  Assert $ λ δ ρ m, ∀ x, assert_holds δ (P x) ρ m.
 Notation "∀ x .. y , P" :=
   (assert_forall (λ x, .. (assert_forall (λ y, P)) ..)) : assert_scope.
 Definition assert_exist {A} (P : A → assert) : assert :=
-  Assert $ λ ρ m, ∃ x, P x ρ m.
+  Assert $ λ δ ρ m, ∃ x, assert_holds δ (P x) ρ m.
 Notation "∃ x .. y , P" :=
   (assert_exist (λ x, .. (assert_exist (λ y, P)) ..)) : assert_scope.
 
 (** Compatibility of the connectives with respect to order and setoid
 equality. *)
-Instance: Proper ((⊆) ==> impl) assert_as_Prop.
+Instance: Proper (impl ==> (⊆@{δ})) Prop_as_assert.
 Proof. solve_assert. Qed.
-Instance: Proper ((≡) ==> iff) assert_as_Prop.
+Instance: Proper (iff ==> (≡@{δ})) Prop_as_assert.
 Proof. solve_assert. Qed.
-Instance: Proper (impl ==> (⊆)) Prop_as_assert.
+Instance: Proper (flip (⊆@{δ}) ==> (⊆@{δ}) ==> (⊆@{δ})) (→)%A.
 Proof. solve_assert. Qed.
-Instance: Proper (iff ==> (≡)) Prop_as_assert.
+Instance: Proper ((≡@{δ}) ==> (≡@{δ}) ==> (≡@{δ})) (→)%A.
 Proof. solve_assert. Qed.
-Instance: Proper (flip (⊆) ==> (⊆) ==> (⊆)) (→)%A.
+Instance: Proper ((≡@{δ}) ==> (≡@{δ}) ==> (≡@{δ})) (↔)%A.
 Proof. solve_assert. Qed.
-Instance: Proper ((≡) ==> (≡) ==> (≡)) (→)%A.
+Instance: Proper ((≡@{δ}) ==> (≡@{δ}) ==> (≡@{δ})) (∧)%A.
 Proof. solve_assert. Qed.
-Instance: Proper ((≡) ==> (≡) ==> (≡)) (↔)%A.
+Instance: Proper ((⊆@{δ}) ==> (⊆@{δ}) ==> (⊆@{δ})) (∧)%A.
 Proof. solve_assert. Qed.
-Instance: Proper ((≡) ==> (≡) ==> (≡)) (∧)%A.
+Instance: Proper ((≡@{δ}) ==> (≡@{δ}) ==> (≡@{δ})) (∨)%A.
 Proof. solve_assert. Qed.
-Instance: Proper ((⊆) ==> (⊆) ==> (⊆)) (∧)%A.
+Instance: Proper ((⊆@{δ}) ==> (⊆@{δ}) ==> (⊆@{δ})) (∨)%A.
 Proof. solve_assert. Qed.
-Instance: Proper ((≡) ==> (≡) ==> (≡)) (∨)%A.
+Instance: Proper ((≡@{δ}) ==> (≡@{δ})) assert_not.
 Proof. solve_assert. Qed.
-Instance: Proper ((⊆) ==> (⊆) ==> (⊆)) (∨)%A.
+Instance: Proper (flip (⊆@{δ}) ==> (⊆@{δ})) assert_not.
 Proof. solve_assert. Qed.
-Instance: Proper ((≡) ==> (≡)) assert_not.
-Proof. solve_assert. Qed.
-Instance: Proper (flip (⊆) ==> (⊆)) assert_not.
-Proof. solve_assert. Qed.
-Instance: Proper (pointwise_relation _ (≡) ==> (≡)) (@assert_forall A).
+Instance:
+  Proper (pointwise_relation _ (≡@{δ}) ==> (≡@{δ})) (@assert_forall A).
 Proof. unfold pointwise_relation. solve_assert. Qed.
-Instance: Proper (pointwise_relation _ (⊆) ==> (⊆)) (@assert_forall A).
+Instance:
+  Proper (pointwise_relation _ (⊆@{δ}) ==> (⊆@{δ})) (@assert_forall A).
 Proof. unfold pointwise_relation. solve_assert. Qed.
-Instance: Proper (pointwise_relation _ (≡) ==> (≡)) (@assert_exist A).
+Instance:
+  Proper (pointwise_relation _ (≡@{δ}) ==> (≡@{δ})) (@assert_exist A).
 Proof. unfold pointwise_relation. solve_assert. Qed.
-Instance: Proper (pointwise_relation _ (⊆) ==> (⊆)) (@assert_exist A).
+Instance:
+  Proper (pointwise_relation _ (⊆@{δ}) ==> (⊆@{δ})) (@assert_exist A).
 Proof. unfold pointwise_relation. solve_assert. Qed.
 
 (** Instances of the type classes for stack independence, memory independence,
-and memory extensibility.  *)
+memory extensibility, unlock independence, and function independence.  *)
 Instance Prop_as_assert_stack_indep P : StackIndep (⌜ P ⌝).
 Proof. solve_assert. Qed.
 Instance assert_impl_stack_indep :
@@ -271,105 +348,152 @@ Instance assert_exist_mem_ext A :
   (∀ x : A, MemExt (P x)) → MemExt (assert_exist P).
 Proof. solve_assert. Qed.
 
+Instance Prop_as_assert_unlock_indep P : UnlockIndep (⌜ P ⌝).
+Proof. solve_assert. Qed.
+Instance assert_impl_unlock_indep :
+  UnlockIndep P → UnlockIndep Q → UnlockIndep (P → Q).
+Proof. solve_assert. Qed.
+Instance assert_and_unlock_indep :
+  UnlockIndep P → UnlockIndep Q → UnlockIndep (P ∧ Q).
+Proof. solve_assert. Qed.
+Instance assert_or_unlock_indep :
+  UnlockIndep P → UnlockIndep Q → UnlockIndep (P ∨ Q).
+Proof. solve_assert eauto. Qed.
+Instance assert_not_unlock_indep :
+  UnlockIndep P → UnlockIndep (¬P).
+Proof. solve_assert. Qed.
+Instance assert_forall_unlock_indep A :
+  (∀ x : A, UnlockIndep (P x)) → UnlockIndep (assert_forall P).
+Proof. solve_assert. Qed.
+Instance assert_exist_unlock_indep A :
+  (∀ x : A, UnlockIndep (P x)) → UnlockIndep (assert_exist P).
+Proof. solve_assert. Qed.
+Instance assert_iff_unlock_indep :
+  UnlockIndep P → UnlockIndep Q → UnlockIndep (P ↔ Q).
+Proof. solve_assert eauto. Qed.
+
+Instance Prop_as_assert_fun_indep P : FunIndep fs (⌜ P ⌝).
+Proof. solve_assert. Qed.
+Instance assert_impl_fun_indep :
+  FunIndep fs P → FunIndep fs Q → FunIndep fs (P → Q).
+Proof. solve_assert eauto. Qed.
+Instance assert_and_fun_indep :
+  FunIndep fs P → FunIndep fs Q → FunIndep fs (P ∧ Q).
+Proof. solve_assert eauto. Qed.
+Instance assert_or_fun_indep :
+  FunIndep fs P → FunIndep fs Q → FunIndep fs (P ∨ Q).
+Proof. solve_assert eauto. Qed.
+Instance assert_not_fun_indep :
+  FunIndep fs P → FunIndep fs (¬P).
+Proof. solve_assert eauto. Qed.
+Instance assert_forall_fun_indep A :
+  (∀ x : A, FunIndep fs (P x)) → FunIndep fs (assert_forall P).
+Proof. solve_assert eauto. Qed.
+Instance assert_exist_fun_indep A :
+  (∀ x : A, FunIndep fs (P x)) → FunIndep fs (assert_exist P).
+Proof. solve_assert eauto. Qed.
+Instance assert_iff_fun_indep :
+  FunIndep fs P → FunIndep fs Q → FunIndep fs (P ↔ Q).
+Proof. unfold assert_iff. apply _. Qed.
+
 (** Proofs of other useful properties. *)
-Instance: Commutative (≡) (↔)%A.
+Instance: Commutative (≡@{δ}) (↔)%A.
 Proof. solve_assert. Qed.
-Instance: Commutative (≡) (∧)%A.
+Instance: Commutative (≡@{δ}) (∧)%A.
 Proof. solve_assert. Qed.
-Instance: Associative (≡) (∧)%A.
+Instance: Associative (≡@{δ}) (∧)%A.
 Proof. solve_assert. Qed.
-Instance: Idempotent (≡) (∧)%A.
+Instance: Idempotent (≡@{δ}) (∧)%A.
 Proof. solve_assert. Qed.
-Instance: Commutative (≡) (∨)%A.
+Instance: Commutative (≡@{δ}) (∨)%A.
 Proof. solve_assert. Qed.
-Instance: Associative (≡) (∨)%A.
+Instance: Associative (≡@{δ}) (∨)%A.
 Proof. solve_assert. Qed.
-Instance: Idempotent (≡) (∨)%A.
+Instance: Idempotent (≡@{δ}) (∨)%A.
 Proof. solve_assert. Qed.
 
-Instance: LeftId (≡) True%A (∧)%A.
+Instance: LeftId (≡@{δ}) True%A (∧)%A.
 Proof. solve_assert. Qed.
-Instance: RightId (≡) True%A (∧)%A.
+Instance: RightId (≡@{δ}) True%A (∧)%A.
 Proof. solve_assert. Qed.
-Instance: LeftAbsorb (≡) False%A (∧)%A.
+Instance: LeftAbsorb (≡@{δ}) False%A (∧)%A.
 Proof. solve_assert. Qed.
-Instance: RightAbsorb (≡) False%A (∧)%A.
+Instance: RightAbsorb (≡@{δ}) False%A (∧)%A.
 Proof. solve_assert. Qed.
-Instance: RightAbsorb (≡) True%A assert_impl.
+Instance: RightAbsorb (≡@{δ}) True%A assert_impl.
 Proof. intros ?. solve_assert. Qed.
-Instance: LeftId (≡) False%A (∨)%A.
+Instance: LeftId (≡@{δ}) False%A (∨)%A.
 Proof. solve_assert. Qed.
-Instance: RightId (≡) False%A (∨)%A.
+Instance: RightId (≡@{δ}) False%A (∨)%A.
 Proof. solve_assert. Qed.
-Instance: LeftAbsorb (≡) True%A (∨)%A.
+Instance: LeftAbsorb (≡@{δ}) True%A (∨)%A.
 Proof. solve_assert. Qed.
-Instance: RightAbsorb (≡) True%A (∨)%A.
+Instance: RightAbsorb (≡@{δ}) True%A (∨)%A.
 Proof. solve_assert. Qed.
 
-Instance: LeftId (≡) True%A (→)%A.
+Instance: LeftId (≡@{δ}) True%A (→)%A.
 Proof. solve_assert. Qed.
-Instance: RightAbsorb (≡) True%A (→)%A.
+Instance: RightAbsorb (≡@{δ}) True%A (→)%A.
 Proof. intros ?. solve_assert. Qed.
 
-Lemma Prop_as_assert_impl (P Q : Prop) : ⌜ P → Q ⌝%A ≡ (⌜P⌝ → ⌜Q⌝)%A.
+Lemma Prop_as_assert_impl (P Q : Prop) δ : ⌜ P → Q ⌝%A ≡@{δ} (⌜P⌝ → ⌜Q⌝)%A.
 Proof. solve_assert. Qed.
-Lemma Prop_as_assert_not (P : Prop) : ⌜ ¬P ⌝%A ≡ (¬⌜P⌝)%A.
+Lemma Prop_as_assert_not (P : Prop) δ : ⌜ ¬P ⌝%A ≡@{δ} (¬⌜P⌝)%A.
 Proof. solve_assert. Qed.
-Lemma Prop_as_assert_and (P Q : Prop) : ⌜ P ∧ Q ⌝%A ≡ (⌜P⌝ ∧ ⌜Q⌝)%A.
+Lemma Prop_as_assert_and (P Q : Prop) δ : ⌜ P ∧ Q ⌝%A ≡@{δ} (⌜P⌝ ∧ ⌜Q⌝)%A.
 Proof. solve_assert. Qed.
-Lemma Prop_as_assert_or (P Q : Prop) : ⌜ P ∨ Q ⌝%A ≡ (⌜P⌝ ∨ ⌜Q⌝)%A.
-Proof. solve_assert. Qed.
-
-Lemma assert_true_intro (P : assert) : P ⊆ True%A.
-Proof. solve_assert. Qed.
-Lemma assert_false_elim (P : assert) : False%A ⊆ P.
+Lemma Prop_as_assert_or (P Q : Prop) δ : ⌜ P ∨ Q ⌝%A ≡@{δ} (⌜P⌝ ∨ ⌜Q⌝)%A.
 Proof. solve_assert. Qed.
 
-Lemma assert_and_l (P Q : assert) : (P ∧ Q)%A ⊆ P.
+Lemma assert_true_intro P δ : P ⊆@{δ} True%A.
 Proof. solve_assert. Qed.
-Lemma assert_and_r (P Q : assert) : (P ∧ Q)%A ⊆ Q.
-Proof. solve_assert. Qed.
-Lemma assert_and_intro P Q1 Q2 : P ⊆ Q1 → P ⊆ Q2 → P ⊆ (Q1 ∧ Q2)%A.
-Proof. solve_assert. Qed.
-Lemma assert_and_elim_l P1 P2 Q : P1 ⊆ Q → (P1 ∧ P2)%A ⊆ Q.
-Proof. solve_assert. Qed.
-Lemma assert_and_elim_r P1 P2 Q : P2 ⊆ Q → (P1 ∧ P2)%A ⊆ Q.
+Lemma assert_false_elim P δ : False%A ⊆@{δ} P.
 Proof. solve_assert. Qed.
 
-Lemma assert_forall_intro {A} P (Q : A → assert) :
-  (∀ x, P ⊆ Q x) → P ⊆ (∀ x, Q x)%A.
+Lemma assert_and_l P Q δ : (P ∧ Q)%A ⊆@{δ} P.
 Proof. solve_assert. Qed.
-Lemma assert_forall_specialize {A} (P : A → assert) Q x :
-  (P x ⊆ Q) → (∀ x, P x)%A ⊆ Q.
+Lemma assert_and_r P Q δ : (P ∧ Q)%A ⊆@{δ} Q.
 Proof. solve_assert. Qed.
-
-Lemma assert_exists_intro {A} P (Q : A → assert) x :
-  P ⊆ Q x → P ⊆ (∃ x, Q x)%A.
+Lemma assert_and_intro P Q1 Q2 δ : P ⊆@{δ} Q1 → P ⊆@{δ} Q2 → P ⊆@{δ} (Q1 ∧ Q2)%A.
 Proof. solve_assert. Qed.
-Lemma assert_exists_elim {A} (P : A → assert) Q :
-  (∀ x, P x ⊆ Q) → (∃ x, P x)%A ⊆ Q.
+Lemma assert_and_elim_l P1 P2 Q δ : P1 ⊆@{δ} Q → (P1 ∧ P2)%A ⊆@{δ} Q.
+Proof. solve_assert. Qed.
+Lemma assert_and_elim_r P1 P2 Q δ : P2 ⊆@{δ} Q → (P1 ∧ P2)%A ⊆@{δ} Q.
 Proof. solve_assert. Qed.
 
-Lemma assert_or_l (P Q : assert) : P ⊆ (P ∨ Q)%A.
+Lemma assert_forall_intro {A} P (Q : A → assert) δ :
+  (∀ x, P ⊆@{δ} Q x) → P ⊆@{δ} (∀ x, Q x)%A.
 Proof. solve_assert. Qed.
-Lemma assert_or_r (P Q : assert) : P ⊆ (P ∨ Q)%A.
-Proof. solve_assert. Qed.
-Lemma assert_or_elim (P Q R : assert) :
-  P ⊆ R → Q ⊆ R → (P ∨ Q)%A ⊆ R.
-Proof. solve_assert. Qed.
-
-Lemma assert_and_exists {A} P (Q : A → assert) :
-  (P ∧ ∃ x, Q x)%A ≡ (∃ x, P ∧ Q x)%A.
-Proof. solve_assert. Qed.
-Lemma assert_exists_and {A} (P : A → assert) Q :
-  ((∃ x, P x) ∧ Q)%A ≡ (∃ x, P x ∧ Q)%A.
+Lemma assert_forall_specialize {A} (P : A → assert) Q δ x :
+  (P x ⊆@{δ} Q) → (∀ x, P x)%A ⊆@{δ} Q.
 Proof. solve_assert. Qed.
 
-Lemma assert_and_exists_l {A} P (Q : A → assert) :
-  (P ∧ ∃ x, Q x)%A ≡ (∃ x, P ∧ Q x)%A.
+Lemma assert_exists_intro {A} P (Q : A → assert) δ x :
+  P ⊆@{δ} Q x → P ⊆@{δ} (∃ x, Q x)%A.
 Proof. solve_assert. Qed.
-Lemma assert_and_exists_r {A} (P : A → assert) Q :
-  ((∃ x, P x) ∧ Q)%A ≡ (∃ x, P x ∧ Q)%A.
+Lemma assert_exists_elim {A} (P : A → assert) Q δ :
+  (∀ x, P x ⊆@{δ} Q) → (∃ x, P x)%A ⊆@{δ} Q.
+Proof. solve_assert. Qed.
+
+Lemma assert_or_l P Q δ : P ⊆@{δ} (P ∨ Q)%A.
+Proof. solve_assert. Qed.
+Lemma assert_or_r P Q δ : P ⊆@{δ} (P ∨ Q)%A.
+Proof. solve_assert. Qed.
+Lemma assert_or_elim P Q R δ : P ⊆@{δ} R → Q ⊆@{δ} R → (P ∨ Q)%A ⊆@{δ} R.
+Proof. solve_assert. Qed.
+
+Lemma assert_and_exists {A} P (Q : A → assert) δ :
+  (P ∧ ∃ x, Q x)%A ≡@{δ} (∃ x, P ∧ Q x)%A.
+Proof. solve_assert. Qed.
+Lemma assert_exists_and {A} (P : A → assert) Q δ :
+  ((∃ x, P x) ∧ Q)%A ≡@{δ} (∃ x, P x ∧ Q)%A.
+Proof. solve_assert. Qed.
+
+Lemma assert_and_exists_l {A} P (Q : A → assert) δ :
+  (P ∧ ∃ x, Q x)%A ≡@{δ} (∃ x, P ∧ Q x)%A.
+Proof. solve_assert. Qed.
+Lemma assert_and_exists_r {A} (P : A → assert) Q δ :
+  ((∃ x, P x) ∧ Q)%A ≡@{δ} (∃ x, P x ∧ Q)%A.
 Proof. solve_assert. Qed.
 
 (** The assertion [e ⇓ v] asserts that the expression [e] evaluates to [v]
@@ -378,7 +502,7 @@ and [e ⇓ -] asserts that the expression [e] evaluates to an arbitrary value
 Notation vassert := (value → assert).
 
 Definition assert_expr (e : expr) : vassert := λ v,
-  Assert $ λ ρ m, ⟦ e ⟧ ρ m = Some v.
+  Assert $ λ δ ρ m, ⟦ e ⟧ δ ρ m = Some v.
 Infix "⇓" := assert_expr (at level 60) : assert_scope.
 Notation "(⇓)" := assert_expr (only parsing) : assert_scope.
 Notation "( e ⇓)" := (assert_expr e) (only parsing) : assert_scope.
@@ -398,36 +522,39 @@ Instance assert_expr_mem_indep e :
   load_free e →
   MemIndep (e ⇓ v).
 Proof.
-  intros ?? ρ m1 m2. unfold_assert.
-  erewrite !(expr_load_free_mem_indep ρ m1 m2); eauto.
+  intros ?? δ ρ m1 m2. unfold_assert.
+  erewrite !(expr_load_free_mem_indep δ ρ m1 m2); eauto.
 Qed.
 Instance assert_expr_mem_indep_ e :
   load_free e →
   MemIndep (e ⇓ -).
 Proof.
-  intros ? ρ m1 m2 [v ?]. exists v. unfold_assert in *.
-  erewrite !(expr_load_free_mem_indep ρ m2 m1); eauto.
+  intros ? δ ρ m1 m2 [v ?]. exists v. unfold_assert in *.
+  erewrite !(expr_load_free_mem_indep δ ρ m2 m1); eauto.
 Qed.
 
 Instance assert_expr_stack_indep e v :
-  expr_vars e ≡ ∅ →
+  vars e ≡ ∅ →
   StackIndep (e ⇓ v).
 Proof.
-  intros ? ρ1 ρ2 m. unfold_assert.
-  by rewrite !(expr_var_free_stack_indep ρ2 ρ1).
+  intros ? δ ρ1 ρ2 m. unfold_assert.
+  by rewrite !(expr_var_free_stack_indep δ ρ2 ρ1).
 Qed.
 Instance assert_expr_stack_indep_ e :
-  expr_vars e ≡ ∅ →
+  vars e ≡ ∅ →
   StackIndep (e ⇓ -).
 Proof.
-  intros ? ρ1 ρ2 m. unfold_assert.
-  by rewrite !(expr_var_free_stack_indep ρ2 ρ1).
+  intros ? δ ρ1 ρ2 m. unfold_assert.
+  by rewrite !(expr_var_free_stack_indep δ ρ2 ρ1).
 Qed.
 
-Lemma assert_expr_load e p v :
-  (load e ⇓ p ∧ load (val p) ⇓ v)%A ⊆ (load (load e) ⇓ v)%A.
-Proof. intros ?? [He ?]. unfold_assert in *. by rewrite He. Qed.
-Lemma assert_expr_forget e v : (e ⇓ v)%A ⊆ (e ⇓ -)%A.
+Lemma assert_expr_load e p v δ :
+  (load e ⇓ p ∧ load (val p) ⇓ v)%A ⊆@{δ} (load (load e) ⇓ v)%A.
+Proof.
+  intros ?? [He ?]. unfold_assert in *. rewrite He.
+  by simplify_option_equality.
+Qed.
+Lemma assert_expr_forget e v δ : (e ⇓ v)%A ⊆@{δ} (e ⇓ -)%A.
 Proof. solve_assert. Qed.
 
 Notation "e ⇓ 'true'" := (∃ v, e⇓v ∧ ⌜ value_true v ⌝)%A
@@ -441,31 +568,31 @@ Definition assert_is_false (Pv : vassert) : assert :=
   (∃ v, Pv v ∧ ⌜ value_false v ⌝)%A.
 
 Definition assert_subst (a : index) (v : value) (P : assert) :=
-  Assert $ λ ρ m, P ρ (<[a:=v]>m).
+  Assert $ λ δ ρ m, assert_holds δ P ρ (<[a:=v]>m).
 Notation "<[ a := v ]>" := (assert_subst a v) : assert_scope.
 
-Instance: ∀ a v, Proper ((≡) ==> (≡)) (assert_subst a v).
+Instance: ∀ a v, Proper ((≡@{δ}) ==> (≡@{δ})) (assert_subst a v).
 Proof. solve_assert. Qed.
 
-Lemma assert_subst_mem_indep P `{MemIndep P} a v:
-  (<[a:=v]>P)%A ≡ P.
+Lemma assert_subst_mem_indep P `{MemIndep P} δ a v:
+  (<[a:=v]>P)%A ≡@{δ} P.
 Proof. solve_assert. Qed.
-Lemma assert_subst_impl P Q a v :
-  (<[a:=v]>(P → Q))%A ≡ (<[a:=v]>P → <[a:=v]>Q)%A.
+Lemma assert_subst_impl P Q δ a v :
+  (<[a:=v]>(P → Q))%A ≡@{δ} (<[a:=v]>P → <[a:=v]>Q)%A.
 Proof. solve_assert. Qed.
-Lemma assert_subst_not P a v : (<[a:=v]>(¬P))%A ≡ (¬<[a:=v]>P)%A.
+Lemma assert_subst_not P δ a v : (<[a:=v]>(¬P))%A ≡@{δ} (¬<[a:=v]>P)%A.
 Proof. solve_assert. Qed.
-Lemma assert_subst_and P Q a v :
-  (<[a:=v]>(P ∧ Q))%A ≡ (<[a:=v]>P ∧ <[a:=v]>Q)%A.
+Lemma assert_subst_and P Q δ a v :
+  (<[a:=v]>(P ∧ Q))%A ≡@{δ} (<[a:=v]>P ∧ <[a:=v]>Q)%A.
 Proof. solve_assert. Qed.
-Lemma assert_subst_or P Q a v :
-  (<[a:=v]>(P ∨ Q))%A ≡ (<[a:=v]>P ∨ <[a:=v]>Q)%A.
+Lemma assert_subst_or P Q δ a v :
+  (<[a:=v]>(P ∨ Q))%A ≡@{δ} (<[a:=v]>P ∨ <[a:=v]>Q)%A.
 Proof. solve_assert. Qed.
-Lemma assert_subst_forall `(P : A → assert) a v :
-  (<[a:=v]>(∀ x, P x))%A ≡ (∀ x, <[a:=v]>(P x))%A.
+Lemma assert_subst_forall {A} (P : A → assert) δ a v :
+  (<[a:=v]>(∀ x, P x))%A ≡@{δ} (∀ x, <[a:=v]>(P x))%A.
 Proof. solve_assert. Qed.
-Lemma assert_subst_exists `(P : A → assert) a v :
-  (<[a:=v]>(∃ x, P x))%A ≡ (∃ x, <[a:=v]>(P x))%A.
+Lemma assert_subst_exists {A} (P : A → assert) δ a v :
+  (<[a:=v]>(∃ x, P x))%A ≡@{δ} (∃ x, <[a:=v]>(P x))%A.
 Proof. solve_assert. Qed.
 
 (** * Separation logic connectives *)
@@ -475,18 +602,20 @@ disjoint parts such that [P] holds in the one part, and [Q] in the other.
 The assertion [P -★ Q] (called separating implication or magic wand) asserts
 that if an arbitrary memory is extended with a disjoint part in which [P]
 holds, then [Q] holds in the extended memory. *)
-Definition assert_emp : assert := Assert $ λ ρ m, m = ∅.
+Definition assert_emp : assert := Assert $ λ δ ρ m, m = ∅.
 Notation "'emp'" := assert_emp : assert_scope.
 
 Definition assert_sep (P Q : assert) : assert :=
-  Assert $ λ ρ m, ∃ m1 m2, m1 ∪ m2 = m ∧ m1 ⊥ m2 ∧ P ρ m1 ∧ Q ρ m2.
+  Assert $ λ δ ρ m, ∃ m1 m2,
+    m1 ∪ m2 = m ∧ m1 ⊥ m2 ∧ assert_holds δ P ρ m1 ∧ assert_holds δ Q ρ m2.
 Infix "★" := assert_sep (at level 80, right associativity) : assert_scope.
 Notation "(★)" := assert_sep (only parsing) : assert_scope.
 Notation "( P ★)" := (assert_sep P) (only parsing) : assert_scope.
 Notation "(★ Q )" := (λ P, assert_sep P Q) (only parsing) : assert_scope.
 
 Definition assert_wand (P Q : assert) : assert :=
-  Assert $ λ ρ m1, ∀ m2, m1 ⊥ m2 → P ρ m2 → Q ρ (m1 ∪ m2).
+  Assert $ λ δ ρ m1, ∀ m2,
+    m1 ⊥ m2 → assert_holds δ P ρ m2 → assert_holds δ Q ρ (m1 ∪ m2).
 Infix "-★" := assert_wand (at level 90) : assert_scope.
 Notation "(-★)" := assert_wand (only parsing) : assert_scope.
 Notation "( P -★)" := (assert_wand P) (only parsing) : assert_scope.
@@ -494,46 +623,46 @@ Notation "(-★ Q )" := (λ P, assert_wand P Q) (only parsing) : assert_scope.
 
 (** Compatibility of the separation logic connectives with respect to order and
 equality. *)
-Instance: Proper ((⊆) ==> (⊆) ==> (⊆)) (★)%A.
+Instance: Proper ((⊆@{δ}) ==> (⊆@{δ}) ==> (⊆@{δ})) (★)%A.
 Proof. solve_assert. Qed.
-Instance: Proper ((≡) ==> (≡) ==> (≡)) (★)%A.
+Instance: Proper ((≡@{δ}) ==> (≡@{δ}) ==> (≡@{δ})) (★)%A.
 Proof. solve_assert. Qed.
-Instance: Proper (flip (⊆) ==> (⊆) ==> (⊆)) (-★)%A.
+Instance: Proper (flip (⊆@{δ}) ==> (⊆@{δ}) ==> (⊆@{δ})) (-★)%A.
 Proof. solve_assert. Qed.
-Instance: Proper ((≡) ==> (≡) ==> (≡)) (-★)%A.
+Instance: Proper ((≡@{δ}) ==> (≡@{δ}) ==> (≡@{δ})) (-★)%A.
 Proof. solve_assert. Qed.
 
 (** Basic properties. *)
-Lemma assert_sep_commutative_1 P Q : (P ★ Q)%A ⊆ (Q ★ P)%A.
+Lemma assert_sep_commutative_1 P Q δ : (P ★ Q)%A ⊆@{δ} (Q ★ P)%A.
 Proof.
   intros ρ m (m1 & m2 & ? & ? & HP & HQ); simpl in *.
   exists m2 m1. by rewrite mem_union_commutative.
 Qed.
-Instance: Commutative (≡) (★)%A.
+Instance: Commutative (≡@{δ}) (★)%A.
 Proof. split; apply assert_sep_commutative_1. Qed.
 
-Lemma assert_sep_left_id_1 P : (emp ★ P)%A ⊆ P.
+Lemma assert_sep_left_id_1 P δ : (emp ★ P)%A ⊆@{δ} P.
 Proof.
   intros ρ m (m1 & m2 & H & ? & ? & Hm2). simpl in *.
   unfold_assert in *. subst. by rewrite (left_id_eq ∅ (∪)).
 Qed.
-Lemma assert_sep_left_id_2 P : P ⊆ (emp ★ P)%A.
+Lemma assert_sep_left_id_2 P δ : P ⊆@{δ} (emp ★ P)%A.
 Proof.
   intros ? m ?. exists (∅ : mem) m. unfold_assert. split_ands; auto.
   * apply (left_id _ _).
   * apply mem_disjoint_empty_l.
 Qed.
-Instance: LeftId (≡) emp%A (★)%A.
+Instance: LeftId (≡@{δ}) emp%A (★)%A.
 Proof. split. apply assert_sep_left_id_1. apply assert_sep_left_id_2. Qed.
-Instance: RightId (≡) emp%A (★)%A.
-Proof. intros ?. by rewrite (commutative _), (left_id _ _). Qed.
+Instance: RightId (≡@{δ}) emp%A (★)%A.
+Proof. intros ??. by rewrite (commutative _), (left_id _ _). Qed.
 
-Instance: LeftAbsorb (≡) False%A (★)%A.
+Instance: LeftAbsorb (≡@{δ}) False%A (★)%A.
 Proof. solve_assert. Qed.
-Instance: RightAbsorb (≡) False%A (★)%A.
+Instance: RightAbsorb (≡@{δ}) False%A (★)%A.
 Proof. solve_assert. Qed.
 
-Lemma assert_sep_associative_1 P Q R : ((P ★ Q) ★ R)%A ⊆ (P ★ (Q ★ R))%A.
+Lemma assert_sep_associative_1 P Q R δ : ((P ★ Q) ★ R)%A ⊆@{δ} (P ★ (Q ★ R))%A.
 Proof.
   intros ?? (?&mR&?&?& (mP&mQ&?&?&?&?) &?); simpl in *; subst.
   exists mP (mQ ∪ mR). split_ands; auto.
@@ -542,7 +671,7 @@ Proof.
   * exists mQ mR. eauto using mem_disjoint_union_lr.
 Qed.
 
-Lemma assert_sep_associative_2 P Q R : (P ★ (Q ★ R))%A ⊆ ((P ★ Q) ★ R)%A.
+Lemma assert_sep_associative_2 P Q R δ : (P ★ (Q ★ R))%A ⊆@{δ} ((P ★ Q) ★ R)%A.
 Proof.
   intros ?? (mP&?&?&?&?&mQ&mR&?&?&?&?); simpl in *; subst.
   exists (mP ∪ mQ) mR. split_ands; auto.
@@ -550,31 +679,31 @@ Proof.
   * by apply mem_disjoint_union_move_r.
   * exists mP mQ. eauto using mem_disjoint_union_rl.
 Qed.
-Instance: Associative (≡) (★)%A.
+Instance: Associative (≡@{δ}) (★)%A.
 Proof.
   split. apply assert_sep_associative_2. apply assert_sep_associative_1.
 Qed.
 
-Lemma assert_wand_intro (P Q R S : assert) :
-  (P ★ Q)%A ⊆ R →
-  P ⊆ (Q -★ R)%A.
+Lemma assert_wand_intro P Q R δ :
+  (P ★ Q)%A ⊆@{δ} R →
+  P ⊆@{δ} (Q -★ R)%A.
 Proof. solve_assert. Qed.
-Lemma assert_wand_elim (P Q : assert) :
-  (P ★ (P -★ Q))%A ⊆ Q.
+Lemma assert_wand_elim δ P Q :
+  (P ★ (P -★ Q))%A ⊆@{δ} Q.
 Proof. rewrite (commutative (★))%A. solve_assert. Qed.
 
-Lemma assert_and_sep_associative (P Q R : assert) :
+Lemma assert_and_sep_associative P Q R δ :
   MemIndep P →
-  (P ∧ (Q ★ R))%A ≡ ((P ∧ Q) ★ R)%A.
+  (P ∧ (Q ★ R))%A ≡@{δ} ((P ∧ Q) ★ R)%A.
 Proof. solve_assert. Qed.
-Lemma assert_sep_and_associative (P Q R : assert) :
+Lemma assert_sep_and_associative P Q R δ :
   MemIndep R →
-  ((P ★ Q) ∧ R)%A ≡ (P ★ (Q ∧ R))%A.
+  ((P ★ Q) ∧ R)%A ≡@{δ} (P ★ (Q ∧ R))%A.
 Proof. solve_assert. Qed.
 
 (** The separation conjunction allows us to give an alternative formulation
 of memory extensibility. *)
-Lemma mem_ext_sep_true `{MemExt P} : P ≡ (P ★ True)%A.
+Lemma mem_ext_sep_true P `{MemExt P} δ : P ≡@{δ} (P ★ True)%A.
 Proof.
   split.
   * intros ? m ?. exists m (∅ : mem). unfold_assert. split_ands; auto.
@@ -583,19 +712,21 @@ Proof.
   * intros ?? (m1 & m2 & ? & ? & ? & ?). subst.
     apply mem_ext with m1; auto using mem_union_subseteq_l.
 Qed.
-Lemma assert_sep_true_mem_ext P : P ≡ (P ★ True)%A → MemExt P.
+Lemma assert_sep_true_mem_ext P : (∀ δ, P ≡@{δ} (P ★ True)%A) → MemExt P.
 Proof.
-  intros H ρ m1 m2 ??. rewrite H. exists m1 (m2 ∖ m1).
+  intros H δ ρ m1 m2 ??. rewrite H. exists m1 (m2 ∖ m1).
   unfold_assert. split_ands; auto.
   * by rewrite mem_difference_union.
   * by apply mem_difference_disjoint_r.
 Qed.
-Lemma mem_ext_sep_true_iff P : P ≡ (P ★ True)%A ↔ MemExt P.
+Lemma mem_ext_sep_true_iff P : (∀ δ, P ≡@{δ} (P ★ True)%A) ↔ MemExt P.
 Proof. split; auto using @mem_ext_sep_true, assert_sep_true_mem_ext. Qed.
 
 (** Other type class instances for stack independence, memory independence, and
 memory extensibility. *)
 Instance assert_emp_stack_indep : StackIndep emp.
+Proof. solve_assert. Qed.
+Instance assert_emp_fun_indep fs : FunIndep fs emp.
 Proof. solve_assert. Qed.
 Instance assert_sep_stack_indep :
   StackIndep P → StackIndep Q → StackIndep (P ★ Q).
@@ -603,7 +734,7 @@ Proof. solve_assert. Qed.
 Instance assert_sep_mem_indep :
   MemIndep P → MemIndep Q → MemIndep (P ★ Q).
 Proof.
-  intros ???? ? m1 m2 (m2' & m2'' &?&?&?&?). subst.
+  intros ????? ? m1 m2 (m2' & m2'' &?&?&?&?). subst.
   exists m2 (∅ : mem). split_ands.
   * by apply (right_id _ _).
   * apply mem_disjoint_empty_r.
@@ -612,7 +743,7 @@ Proof.
 Qed.
 Instance assert_sep_mem_ext_2 : MemExt Q → MemExt (P ★ Q).
 Proof.
-  intros ??? ? m1 m2 (m2' & m2'' &?&?&?&?) ?. subst.
+  intros ???? ? m1 m2 (m2' & m2'' &?&?&?&?) ?. subst.
   exists m2' (m2'' ∪ m2 ∖ (m2' ∪ m2'')). split_ands; auto.
   * by rewrite (associative _), mem_difference_union.
   * apply mem_disjoint_union_move_l; auto using mem_difference_disjoint_r.
@@ -622,29 +753,35 @@ Proof.
 Qed.
 Instance assert_sep_mem_ext_l : MemExt P → MemExt (P ★ Q).
 Proof.
-  intros P Q ????. rewrite !(commutative (★) P)%A.
+  intros P Q ?????. rewrite !(commutative (★) P)%A.
   by apply assert_sep_mem_ext_2.
 Qed.
+Instance assert_sep_fun_indep :
+  FunIndep fs P → FunIndep fs Q → FunIndep fs (P ★ Q).
+Proof. solve_assert eauto. Qed.
 
 (** Proofs of other useful properties. *)
-Lemma assert_and_sep_emp_l (P Q : assert) :
+Lemma assert_and_sep_emp_l P Q δ :
   MemIndep P →
-  (P ∧ Q)%A ≡ ((P ∧ emp) ★ Q)%A.
+  (P ∧ Q)%A ≡@{δ} ((P ∧ emp) ★ Q)%A.
 Proof.
   intro. by rewrite <-assert_and_sep_associative, (left_id emp (★))%A.
 Qed.
-Lemma assert_and_sep_emp_r (P Q : assert) :
+Lemma assert_and_sep_emp_r P Q δ :
   MemIndep Q →
-  (P ∧ Q)%A ≡ (P ★ (Q ∧ emp))%A.
+  (P ∧ Q)%A ≡@{δ} (P ★ (Q ∧ emp))%A.
 Proof. intro. by rewrite !(commutative _ P), assert_and_sep_emp_l. Qed.
 
-Lemma assert_sep_elim_l P1 P2 Q :
+Lemma assert_sep_elim_l P1 P2 Q δ :
   MemExt Q →
-  P1 ⊆ Q → (P1 ★ P2)%A ⊆ Q.
-Proof. intros ? H. by rewrite mem_ext_sep_true, H, <-assert_true_intro. Qed.
-Lemma assert_sep_elim_r P1 P2 Q :
+  P1 ⊆@{δ} Q → (P1 ★ P2)%A ⊆@{δ} Q.
+Proof.
+  intros ? H.
+  by rewrite (mem_ext_sep_true Q), H, <-assert_true_intro.
+Qed.
+Lemma assert_sep_elim_r P1 P2 Q δ :
   MemExt Q →
-  P2 ⊆ Q → (P1 ★ P2)%A ⊆ Q.
+  P2 ⊆@{δ} Q → (P1 ★ P2)%A ⊆@{δ} Q.
 Proof. rewrite (commutative (★))%A. apply assert_sep_elim_l. Qed.
 
 (** The assertion [Π Ps] states that the memory can be split into disjoint
@@ -654,24 +791,24 @@ Definition assert_sep_list : list assert → assert :=
 Notation "'Π' Ps" := (assert_sep_list Ps)
   (at level 20, format "Π  Ps") : assert_scope.
 
-Instance: Proper (eqlistA (≡) ==> (≡)) assert_sep_list.
+Instance: Proper (eqlistA (≡@{δ}) ==> (≡@{δ})) assert_sep_list.
 Proof. induction 1; simpl; by f_equiv. Qed.
 
-Lemma assert_sep_list_alt_2 (Ps : list assert) ρ ms :
+Lemma assert_sep_list_alt_2 (Ps : list assert) δ ρ ms :
   list_disjoint ms →
-  Forall2 (λ (P : assert) m, P ρ m) Ps ms →
-  (Π Ps)%A ρ (⋃ ms).
+  Forall2 (λ (P : assert) m, assert_holds δ P ρ m) Ps ms →
+  assert_holds δ (Π Ps)%A ρ (⋃ ms).
 Proof.
   intros Hms HPs. revert Hms.
   induction HPs as [|P m Ps ms IH]; inversion_clear 1.
   + done.
   + exists m (⋃ ms); simpl; auto.
 Qed.
-Lemma assert_sep_list_alt (Ps : list assert) ρ m :
-  (Π Ps)%A ρ m ↔ ∃ ms,
+Lemma assert_sep_list_alt (Ps : list assert) δ ρ m :
+  assert_holds δ (Π Ps)%A ρ m ↔ ∃ ms,
     m = ⋃ ms
   ∧ list_disjoint ms
-  ∧ Forall2 (λ (P : assert) m, P ρ m) Ps ms.
+  ∧ Forall2 (λ (P : assert) m, assert_holds δ P ρ m) Ps ms.
 Proof.
   split.
   * revert m. induction Ps as [|P Ps IH].
@@ -684,11 +821,11 @@ Proof.
   * naive_solver auto using assert_sep_list_alt_2.
 Qed.
 
-Lemma assert_sep_list_alt_vec {n} (Ps : vec assert n) ρ m :
-  (Π Ps)%A ρ m ↔ ∃ ms : vec mem n,
+Lemma assert_sep_list_alt_vec {n} (Ps : vec assert n) δ ρ m :
+  assert_holds δ (Π Ps)%A ρ m ↔ ∃ ms : vec mem n,
     m = ⋃ ms
   ∧ list_disjoint ms
-  ∧ ∀ i, (Ps !!! i) ρ (ms !!! i).
+  ∧ ∀ i, assert_holds δ (Ps !!! i) ρ (ms !!! i).
 Proof.
   rewrite assert_sep_list_alt. split.
   * intros (ms & ? & ? & Hms).
@@ -699,54 +836,54 @@ Proof.
     by rewrite <-(vec_to_list_of_list ms), Forall2_vlookup in Hms.
   * intros [ms ?]. exists ms. by rewrite Forall2_vlookup.
 Qed.
-Lemma assert_sep_list_alt_vec_2 {n} (Ps : vec assert n) ρ (ms : vec mem n) :
+Lemma assert_sep_list_alt_vec_2 {n} (Ps : vec assert n) δ ρ (ms : vec mem n) :
   list_disjoint ms →
-  (∀ i, (Ps !!! i) ρ (ms !!! i)) →
-  (Π Ps)%A ρ (⋃ ms).
+  (∀ i, assert_holds δ (Ps !!! i) ρ (ms !!! i)) →
+  assert_holds δ (Π Ps)%A ρ (⋃ ms).
 Proof. intros. apply assert_sep_list_alt_vec. eauto. Qed.
 
 (** The assertion [e1 ↦{γ} e2] asserts that the memory consists of exactly one
 cell at address [e1] with permission [γ] and contents [e2]. The assertion
-[e1 ↦{γ} -] asserts that the memory consists of exactly one cell at address [e1]
-with permission [γ] and arbitrary contents. *)
+[e1 ↦{γ} -] asserts that the memory consists of exactly one cell at address
+[e1] with permission [γ] and arbitrary contents. *)
 Definition assert_singleton (e1 e2 : expr) (γ : memperm) : assert :=
-  Assert $ λ ρ m, ∃ a v,
-    ⟦ e1 ⟧ ρ m = Some (ptr a)%V ∧ ⟦ e2 ⟧ ρ m = Some v ∧ m = {[(a,v,γ)]}.
+  Assert $ λ δ ρ m, ∃ a v,
+    ⟦ e1 ⟧ δ ρ m = Some (ptr a)%V ∧ ⟦ e2 ⟧ δ ρ m = Some v ∧ m = {[(a,v,γ)]}.
 Notation "e1 ↦{ γ } e2" := (assert_singleton e1 e2 γ)%A
   (at level 20, format "e1  ↦{ γ }  e2") : assert_scope.
 Definition assert_singleton_ (e : expr) (γ : memperm) : assert :=
-  Assert $ λ ρ m, ∃ a v,
-    ⟦ e ⟧ ρ m = Some (ptr a)%V ∧ m = {[(a,v,γ)]}.
+  Assert $ λ δ ρ m, ∃ a v,
+    ⟦ e ⟧ δ ρ m = Some (ptr a)%V ∧ m = {[(a,v,γ)]}.
 Notation "e ↦{ γ } -" := (assert_singleton_ e γ)%A
   (at level 20, format "e  ↦{ γ }  -") : assert_scope.
 
-Lemma assert_singleton_forget e1 e2 γ : (e1 ↦{γ} e2)%A ⊆ (e1 ↦{γ} -)%A.
+Lemma assert_singleton_forget δ e1 e2 γ : (e1 ↦{γ} e2)%A ⊆@{δ} (e1 ↦{γ} -)%A.
 Proof. solve_assert. Qed.
 
 Instance assert_singleton_stack_indep e1 e2 γ :
-  expr_vars e1 ≡ ∅ →
-  expr_vars e2 ≡ ∅ →
+  vars e1 ≡ ∅ →
+  vars e2 ≡ ∅ →
   StackIndep (e1 ↦{γ} e2).
 Proof.
-  intros ?? ρ1 ρ2 m (a & v & ?). exists a v.
-  by rewrite !(expr_var_free_stack_indep ρ2 ρ1).
+  intros ?? δ ρ1 ρ2 m (a & v & ?). exists a v.
+  by rewrite !(expr_var_free_stack_indep δ ρ2 ρ1).
 Qed.
 Instance assert_singleton_stack_indep_ e γ :
-  expr_vars e ≡ ∅ →
+  vars e ≡ ∅ →
   StackIndep (e ↦{γ} -).
 Proof.
-  intros ? ρ1 ρ2 m (a&v&?). exists a v.
-  by rewrite !(expr_var_free_stack_indep ρ2 ρ1).
+  intros ? δ ρ1 ρ2 m (a&v&?). exists a v.
+  by rewrite !(expr_var_free_stack_indep δ ρ2 ρ1).
 Qed.
 
-Lemma assert_singleton_eval_l e1 v1 e2 γ :
-  (e1 ⇓ v1 ∧ val v1 ↦{γ} e2)%A ⊆ (e1 ↦{γ} e2)%A.
+Lemma assert_singleton_eval_l δ e1 v1 e2 γ :
+  (e1 ⇓ v1 ∧ val v1 ↦{γ} e2)%A ⊆@{δ} (e1 ↦{γ} e2)%A.
 Proof. solve_assert. Qed.
-Lemma assert_singleton_eval_r e1 v2 e2 γ :
-  (e1 ↦{γ} val v2 ∧ e2 ⇓ v2)%A ⊆ (e1 ↦{γ} e2)%A.
+Lemma assert_singleton_eval_r δ e1 v2 e2 γ :
+  (e1 ↦{γ} val v2 ∧ e2 ⇓ v2)%A ⊆@{δ} (e1 ↦{γ} e2)%A.
 Proof. solve_assert. Qed.
-Lemma assert_singleton_eval_ e v γ :
-  (e ⇓ v ∧ val v ↦{γ} -)%A ⊆ (e ↦{γ} -)%A.
+Lemma assert_singleton_eval_ δ e v γ :
+  (e ⇓ v ∧ val v ↦{γ} -)%A ⊆@{δ} (e ↦{γ} -)%A.
 Proof. solve_assert. Qed.
 
 (** The assertion [e1 ↪{γ} e2] asserts that the memory contains at least one
@@ -754,70 +891,70 @@ cell at address [e1] with permission [γ] and contents [e2]. The assertion
 [e1 ↪{γ} -] asserts that the memory contains at least one cell at address
 [e1] with permission [γ] and arbitrary contents. *)
 Definition assert_assign (e1 e2 : expr) (γ : memperm) : assert :=
-  Assert $ λ ρ m, ∃ a v,
-    ⟦ e1 ⟧ ρ m = Some (ptr a)%V ∧
-    ⟦ e2 ⟧ ρ m = Some v ∧
+  Assert $ λ δ ρ m, ∃ a v,
+    ⟦ e1 ⟧ δ ρ m = Some (ptr a)%V ∧
+    ⟦ e2 ⟧ δ ρ m = Some v ∧
     {[(a,v,γ)]} ⊆ m.
 Notation "e1 ↪{ γ } e2" := (assert_assign e1 e2 γ)%A
   (at level 20, format "e1  ↪{ γ }  e2") : assert_scope.
 Definition assert_assign_ (e : expr) (γ : memperm) : assert :=
-  Assert $ λ ρ m, ∃ a v,
-    ⟦ e ⟧ ρ m = Some (ptr a)%V ∧
+  Assert $ λ δ ρ m, ∃ a v,
+    ⟦ e ⟧ δ ρ m = Some (ptr a)%V ∧
     {[(a,v,γ)]} ⊆ m.
 Notation "e ↪{ γ } -" := (assert_assign_ e γ)%A
   (at level 20, format "e  ↪{ γ }  -") : assert_scope.
 
-Lemma assert_assign_forget e1 e2 γ : (e1 ↪{γ} e2)%A ⊆ (e1 ↪{γ} -)%A.
+Lemma assert_assign_forget δ e1 e2 γ : (e1 ↪{γ} e2)%A ⊆@{δ} (e1 ↪{γ} -)%A.
 Proof. solve_assert. Qed.
-Lemma assert_singleton_assign e1 e2 γ : (e1 ↦{γ} e2)%A ⊆ (e1 ↪{γ} e2)%A.
+Lemma assert_singleton_assign δ e1 e2 γ : (e1 ↦{γ} e2)%A ⊆@{δ} (e1 ↪{γ} e2)%A.
 Proof. solve_assert. Qed.
-Lemma assert_singleton_assign_ e γ : (e ↦{γ} -)%A ⊆ (e ↪{γ} -)%A.
+Lemma assert_singleton_assign_ δ e γ : (e ↦{γ} -)%A ⊆@{δ} (e ↪{γ} -)%A.
 Proof. solve_assert. Qed.
 
-Lemma assert_assign_eval_l e1 v1 e2 γ :
-  (e1 ⇓ v1 ∧ val v1 ↪{γ} e2)%A ⊆ (e1 ↪{γ} e2)%A.
+Lemma assert_assign_eval_l δ e1 v1 e2 γ :
+  (e1 ⇓ v1 ∧ val v1 ↪{γ} e2)%A ⊆@{δ} (e1 ↪{γ} e2)%A.
 Proof. solve_assert. Qed.
-Lemma assert_assign_eval_r e1 v2 e2 γ :
-  (e1 ↪{γ} val v2 ∧ e2 ⇓ v2)%A ⊆ (e1 ↪{γ} e2)%A.
+Lemma assert_assign_eval_r δ e1 v2 e2 γ :
+  (e1 ↪{γ} val v2 ∧ e2 ⇓ v2)%A ⊆@{δ} (e1 ↪{γ} e2)%A.
 Proof. solve_assert. Qed.
-Lemma assert_assign_eval_ e v γ :
-  (e ⇓ v ∧ val v ↪{γ} -)%A ⊆ (e ↪{γ} -)%A.
+Lemma assert_assign_eval_ δ e v γ :
+  (e ⇓ v ∧ val v ↪{γ} -)%A ⊆@{δ} (e ↪{γ} -)%A.
 Proof. solve_assert. Qed.
 
 Instance assert_assign_stack_indep e1 e2 γ :
-  expr_vars e1 ≡ ∅ →
-  expr_vars e2 ≡ ∅ →
+  vars e1 ≡ ∅ →
+  vars e2 ≡ ∅ →
   StackIndep (e1 ↪{γ} e2).
 Proof.
-  intros ?? ρ1 ρ2 m (a&v&γ'&?). exists a v.
-  by rewrite !(expr_var_free_stack_indep ρ2 ρ1).
+  intros ?? δ ρ1 ρ2 m (a&v&γ'&?). exists a v.
+  by rewrite !(expr_var_free_stack_indep δ ρ2 ρ1).
 Qed.
 Instance assert_assign_stack_indep_ e γ :
-  expr_vars e ≡ ∅ →
+  vars e ≡ ∅ →
   StackIndep (e ↪{γ} -).
 Proof.
-  intros ? ρ1 ρ2 m (a&v&γ'&?). exists a v.
-  by rewrite !(expr_var_free_stack_indep ρ2 ρ1).
+  intros ? δ ρ1 ρ2 m (a&v&γ'&?). exists a v.
+  by rewrite !(expr_var_free_stack_indep δ ρ2 ρ1).
 Qed.
 
 Instance assert_assign_mem_ext e1 e2 γ :
   MemExt (e1 ↪{γ} e2).
 Proof.
-  intros ρ m1 m2 (a&v&γ2&?&?) Hm12.
+  intros δ ρ m1 m2 (a&v&γ2&?&?) Hm12.
   exists a v. split_ands; eauto using expr_eval_weaken_mem.
   by transitivity m1.
 Qed.
 Instance assert_assign_mem_ext_ e γ :
   MemExt (e ↪{γ} -).
 Proof.
-  intros ρ m1 m2 (a&v&γ2&?) Hm12.
+  intros δ ρ m1 m2 (a&v&γ2&?) Hm12.
   exists a v. split_ands; eauto using expr_eval_weaken_mem.
   by transitivity m1.
 Qed.
 
-Lemma assign_assign_alt e1 e2 γ :
+Lemma assign_assign_alt δ e1 e2 γ :
   load_free e1 → load_free e2 →
-  (e1 ↪{γ} e2)%A ≡ (e1 ↦{γ} e2 ★ True)%A.
+  (e1 ↪{γ} e2)%A ≡@{δ} (e1 ↦{γ} e2 ★ True)%A.
 Proof.
   split.
   * intros ρ m (a&v&γ'&?&?).
@@ -825,13 +962,13 @@ Proof.
     + by apply mem_difference_union.
     + by apply mem_difference_disjoint_r.
     + exists a v.
-      erewrite !(expr_load_free_mem_indep _ {[(a,v,γ)]} m); eauto.
+      erewrite !(expr_load_free_mem_indep _ _ {[(a,v,γ)]} m); eauto.
     + done.
-  * rewrite assert_singleton_assign. apply mem_ext_sep_true.
+  * rewrite assert_singleton_assign. apply (mem_ext_sep_true _).
 Qed.
-Lemma assert_assign_assign_alt_ e γ :
+Lemma assert_assign_assign_alt_ δ e γ :
   load_free e →
-  (e ↪{γ} -)%A ≡ (e ↦{γ} - ★ True)%A.
+  (e ↪{γ} -)%A ≡@{δ} (e ↦{γ} - ★ True)%A.
 Proof.
   split.
   * intros ρ m (a&v&γ'&?).
@@ -839,23 +976,23 @@ Proof.
     + by apply mem_difference_union.
     + by apply mem_difference_disjoint_r.
     + exists a v. simpl.
-      erewrite !(expr_load_free_mem_indep _ {[(a,v,γ)]} m); eauto.
+      erewrite !(expr_load_free_mem_indep _ _ {[(a,v,γ)]} m); eauto.
     + done.
-  * rewrite assert_singleton_assign_. apply mem_ext_sep_true.
+  * rewrite assert_singleton_assign_. apply (mem_ext_sep_true _).
 Qed.
 
-Lemma assert_assign_load e v γ :
+Lemma assert_assign_load δ e v γ :
   perm_kind γ ≠ Locked →
-  (e ↪{γ} val v)%A ⊆ (load e ⇓ v)%A.
+  (e ↪{γ} val v)%A ⊆@{δ} (load e ⇓ v)%A.
 Proof.
   intros ? ρ m (a&v'&Ha&?&?).
   unfold_assert. rewrite Ha. simplify_option_equality.
   apply mem_lookup_weaken with {[(a, v', γ)]}; [|done].
   by apply mem_lookup_singleton.
 Qed.
-Lemma assert_assign_load_ e γ :
+Lemma assert_assign_load_ δ e γ :
   perm_kind γ ≠ Locked →
-  (e ↪{γ} -)%A ⊆ (load e ⇓ -)%A.
+  (e ↪{γ} -)%A ⊆@{δ} (load e ⇓ -)%A.
 Proof.
   intros ? ρ m (a&v'&Ha&?).
   unfold_assert. rewrite Ha. simplify_option_equality.
@@ -863,39 +1000,39 @@ Proof.
   by apply mem_lookup_singleton.
 Qed.
 
-Lemma assert_singleton_load e v γ :
+Lemma assert_singleton_load δ e v γ :
   perm_kind γ ≠ Locked →
-  (e ↦{γ} val v)%A ⊆ (load e ⇓ v)%A.
+  (e ↦{γ} val v)%A ⊆@{δ} (load e ⇓ v)%A.
 Proof.
   intros. rewrite assert_singleton_assign. by apply assert_assign_load.
 Qed.
-Lemma assert_singleton_load_ e γ :
+Lemma assert_singleton_load_ δ e γ :
   perm_kind γ ≠ Locked →
-  (e ↦{γ} -)%A ⊆ (load e ⇓ -)%A.
+  (e ↦{γ} -)%A ⊆@{δ} (load e ⇓ -)%A.
 Proof.
   intros. by rewrite <-assert_assign_load_, assert_singleton_assign_.
 Qed.
 
 Definition assert_unlock (P : assert) : assert :=
-  Assert $ λ ρ m, P ρ (mem_unlock (locks m) m).
+  Assert $ λ δ ρ m, assert_holds δ P ρ (mem_unlock (locks m) m).
 Notation "P ▷" := (assert_unlock P) (at level 20) : assert_scope.
 
-Instance: Proper ((⊆) ==> (⊆)) assert_unlock.
+Instance: Proper ((⊆@{δ}) ==> (⊆@{δ})) assert_unlock.
 Proof. solve_assert. Qed.
-Instance: Proper ((≡) ==> (≡)) assert_unlock.
+Instance: Proper ((≡@{δ}) ==> (≡@{δ})) assert_unlock.
 Proof. solve_assert. Qed.
 
-Lemma assert_unlock_unlock_indep `{UnlockIndep P} : (P ▷)%A ≡ P.
+Lemma assert_unlock_unlock_indep P `{UnlockIndep P} δ : (P ▷)%A ≡@{δ} P.
 Proof. solve_assert. Qed.
-Lemma assert_unlock_impl P Q : ((P → Q) ▷)%A ≡ (P ▷ → Q ▷)%A.
+Lemma assert_unlock_impl P Q δ : ((P → Q) ▷)%A ≡@{δ} (P ▷ → Q ▷)%A.
 Proof. solve_assert. Qed.
-Lemma assert_unlock_not P : ((¬P)▷)%A ≡ (¬P ▷)%A.
+Lemma assert_unlock_not P δ : ((¬P)▷)%A ≡@{δ} (¬P ▷)%A.
 Proof. solve_assert. Qed.
-Lemma assert_unlock_and P Q : ((P ∧ Q) ▷)%A ≡ (P ▷ ∧ Q ▷)%A.
+Lemma assert_unlock_and P Q δ : ((P ∧ Q) ▷)%A ≡@{δ} (P ▷ ∧ Q ▷)%A.
 Proof. solve_assert. Qed.
-Lemma assert_unlock_or P Q : ((P ∨ Q) ▷)%A ≡ (P ▷ ∨ Q ▷)%A.
+Lemma assert_unlock_or P Q δ : ((P ∨ Q) ▷)%A ≡@{δ} (P ▷ ∨ Q ▷)%A.
 Proof. solve_assert. Qed.
-Lemma assert_unlock_sep P Q : (P ▷ ★ Q ▷)%A ⊆ ((P ★ Q) ▷)%A.
+Lemma assert_unlock_sep P Q δ : (P ▷ ★ Q ▷)%A ⊆@{δ} ((P ★ Q) ▷)%A.
 Proof.
   intros ?? (m1&m2&?&?&?&?).
   exists (mem_unlock (locks m1) m1) (mem_unlock (locks m2) m2).
@@ -903,21 +1040,21 @@ Proof.
   * subst. by rewrite mem_unlock_all_union.
   * by apply mem_disjoint_unlock_l, mem_disjoint_unlock_r.
 Qed.
-Lemma assert_unlock_sep_alt P P' Q Q' :
-  P ⊆ (P' ▷)%A →
-  Q ⊆ (Q' ▷)%A →
-  (P ★ Q)%A ⊆ ((P' ★ Q') ▷)%A.
+Lemma assert_unlock_sep_alt P P' Q Q' δ :
+  P ⊆@{δ} (P' ▷)%A →
+  Q ⊆@{δ} (Q' ▷)%A →
+  (P ★ Q)%A ⊆@{δ} ((P' ★ Q') ▷)%A.
 Proof. intros HP HQ. rewrite HP, HQ. apply assert_unlock_sep. Qed.
 
-Lemma assert_unlock_forall `(P : A → assert) :
-  ((∀ x, P x)▷)%A ≡ (∀ x, (P x)▷)%A.
+Lemma assert_unlock_forall {A} (P : A → assert) δ :
+  ((∀ x, P x)▷)%A ≡@{δ} (∀ x, (P x)▷)%A.
 Proof. solve_assert. Qed.
-Lemma assert_unlock_exists `(P : A → assert) :
-  ((∃ x, P x) ▷)%A ≡ (∃ x, (P x)▷)%A.
+Lemma assert_unlock_exists {A} (P : A → assert) δ :
+  ((∃ x, P x) ▷)%A ≡@{δ} (∃ x, (P x)▷)%A.
 Proof. solve_assert. Qed.
 
-Lemma assert_unlock_singleton_ e1 γ :
-  (e1 ↦{γ} -)%A ⊆ ((e1 ↦{perm_unlock γ} -) ▷)%A.
+Lemma assert_unlock_singleton_ δ e1 γ :
+  (e1 ↦{γ} -)%A ⊆@{δ} ((e1 ↦{perm_unlock γ} -) ▷)%A.
 Proof.
   intros ρ m (a&v&?&?). exists a v. split.
   * unfold_assert. eauto using expr_eval_unlock.
@@ -926,30 +1063,31 @@ Qed.
 
 (** The assertion [P↡] asserts that [P] holds if the stack is cleared. This
 connective allows us to specify stack independence in an alternative way. *)
-Definition assert_clear_stack (P : assert) : assert := Assert $ λ _ m, P [] m.
+Definition assert_clear_stack (P : assert) : assert :=
+  Assert $ λ δ _ m, assert_holds δ P [] m.
 Notation "P ↡" := (assert_clear_stack P) (at level 20) : assert_scope.
 
 Instance assert_clear_stack_clear_stack_indep: StackIndep (P↡).
 Proof. solve_assert. Qed.
-Lemma stack_indep_clear_stack `{StackIndep P} : (P↡)%A ≡ P.
+Lemma stack_indep_clear_stack P `{StackIndep P} δ : (P↡)%A ≡@{δ} P.
 Proof. solve_assert. Qed.
-Lemma stack_indep_clear_stack_iff P : StackIndep P ↔ (P↡)%A ≡ P.
-Proof. solve_assert. Qed.
-
-Lemma assert_clear_stack_impl P Q : ((P → Q)↡)%A ≡ (P↡ → Q↡)%A.
-Proof. solve_assert. Qed.
-Lemma assert_clear_stack_not P : ((¬P)↡)%A ≡ (¬P↡)%A.
-Proof. solve_assert. Qed.
-Lemma assert_clear_stack_and P Q : ((P ∧ Q)↡)%A ≡ (P↡ ∧ Q↡)%A.
-Proof. solve_assert. Qed.
-Lemma assert_clear_stack_or P Q : ((P ∨ Q)↡)%A ≡ (P↡ ∨ Q↡)%A.
-Proof. solve_assert. Qed.
-Lemma assert_clear_stack_sep P Q : ((P ★ Q)↡)%A ≡ (P↡ ★ Q↡)%A.
+Lemma stack_indep_clear_stack_iff P : StackIndep P ↔ (∀ δ, (P↡)%A ≡@{δ} P).
 Proof. solve_assert. Qed.
 
-Instance: Proper ((⊆) ==> (⊆)) assert_clear_stack.
+Lemma assert_clear_stack_impl P Q δ : ((P → Q)↡)%A ≡@{δ} (P↡ → Q↡)%A.
 Proof. solve_assert. Qed.
-Instance: Proper ((≡) ==> (≡)) assert_clear_stack.
+Lemma assert_clear_stack_not P δ : ((¬P)↡)%A ≡@{δ} (¬P↡)%A.
+Proof. solve_assert. Qed.
+Lemma assert_clear_stack_and P Q δ : ((P ∧ Q)↡)%A ≡@{δ} (P↡ ∧ Q↡)%A.
+Proof. solve_assert. Qed.
+Lemma assert_clear_stack_or P Q δ : ((P ∨ Q)↡)%A ≡@{δ} (P↡ ∨ Q↡)%A.
+Proof. solve_assert. Qed.
+Lemma assert_clear_stack_sep P Q δ : ((P ★ Q)↡)%A ≡@{δ} (P↡ ★ Q↡)%A.
+Proof. solve_assert. Qed.
+
+Instance: Proper ((⊆@{δ}) ==> (⊆@{δ})) assert_clear_stack.
+Proof. solve_assert. Qed.
+Instance: Proper ((≡@{δ}) ==> (≡@{δ})) assert_clear_stack.
 Proof. solve_assert. Qed.
 
 (** To deal with block scope variables we need to lift an assertion such that
@@ -957,49 +1095,51 @@ the De Bruijn indexes of its variables are increased. We define the lifting
 [P↑] of an assertion [P] semantically, and prove that it indeed behaves as
 expected. *)
 Definition assert_lift (P : assert) : assert :=
-  Assert $ λ ρ m, P (tail ρ) m.
+  Assert $ λ δ ρ m, assert_holds δ P (tail ρ) m.
 Notation "P ↑" := (assert_lift P) (at level 20) : assert_scope.
 
-Lemma assert_lift_expr e v : ((e ⇓ v)↑)%A ≡ ((e↑) ⇓ v)%A.
+Lemma assert_lift_expr δ e v : ((e ⇓ v)↑)%A ≡@{δ} ((e↑) ⇓ v)%A.
 Proof. by split; intros ??; unfold_assert; rewrite expr_eval_lift. Qed.
-Lemma assert_lift_expr_ e : ((e ⇓ -)↑)%A ≡ ((e↑) ⇓ -)%A.
+Lemma assert_lift_expr_ δ e : ((e ⇓ -)↑)%A ≡@{δ} ((e↑) ⇓ -)%A.
 Proof. by split; intros ??; unfold_assert; rewrite expr_eval_lift. Qed.
-Lemma assert_lift_singleton e1 e2 γ :
-  ((e1 ↦{γ} e2)↑)%A ≡ ((e1↑) ↦{γ} (e2↑))%A.
+Lemma assert_lift_singleton δ e1 e2 γ :
+  ((e1 ↦{γ} e2)↑)%A ≡@{δ} ((e1↑) ↦{γ} (e2↑))%A.
 Proof.
   split; intros ??; unfold_assert; intros H.
   * by rewrite !expr_eval_lift.
   * by rewrite !expr_eval_lift in H.
 Qed.
-Lemma assert_lift_singleton_ e γ : ((e ↦{γ} -)↑)%A ≡ ((e↑) ↦{γ} -)%A.
+Lemma assert_lift_singleton_ δ e γ : ((e ↦{γ} -)↑)%A ≡@{δ} ((e↑) ↦{γ} -)%A.
 Proof.
   split; intros ??; unfold_assert; intros H.
   * by rewrite !expr_eval_lift.
   * by rewrite !expr_eval_lift in H.
 Qed.
-Lemma assert_lift_impl P Q : ((P → Q)↑)%A ≡ (P↑ → Q↑)%A.
+Lemma assert_lift_impl P Q δ : ((P → Q)↑)%A ≡@{δ} (P↑ → Q↑)%A.
 Proof. solve_assert. Qed.
-Lemma assert_lift_not P : ((¬P)↑)%A ≡ (¬P↑)%A.
+Lemma assert_lift_not P δ : ((¬P)↑)%A ≡@{δ} (¬P↑)%A.
 Proof. solve_assert. Qed.
-Lemma assert_lift_and P Q : ((P ∧ Q)↑)%A ≡ (P↑ ∧ Q↑)%A.
+Lemma assert_lift_and P Q δ : ((P ∧ Q)↑)%A ≡@{δ} (P↑ ∧ Q↑)%A.
 Proof. solve_assert. Qed.
-Lemma assert_lift_or P Q : ((P ∨ Q)↑)%A ≡ (P↑ ∨ Q↑)%A.
+Lemma assert_lift_or P Q δ : ((P ∨ Q)↑)%A ≡@{δ} (P↑ ∨ Q↑)%A.
 Proof. solve_assert. Qed.
-Lemma assert_lift_sep P Q : ((P ★ Q)↑)%A ≡ (P↑ ★ Q↑)%A.
+Lemma assert_lift_sep P Q δ : ((P ★ Q)↑)%A ≡@{δ} (P↑ ★ Q↑)%A.
 Proof. solve_assert. Qed.
-Lemma assert_lift_forall `(P : A → assert) : ((∀ x, P x)↑)%A ≡ (∀ x, P x↑)%A.
+Lemma assert_lift_forall {A} (P : A → assert) δ :
+  ((∀ x, P x)↑)%A ≡@{δ} (∀ x, P x↑)%A.
 Proof. solve_assert. Qed.
-Lemma assert_lift_exists `(P : A → assert) : ((∃ x, P x)↑)%A ≡ (∃ x, P x↑)%A.
+Lemma assert_lift_exists {A} (P : A → assert) δ :
+  ((∃ x, P x)↑)%A ≡@{δ} (∃ x, P x↑)%A.
 Proof. solve_assert. Qed.
 
-Instance: Proper ((⊆) ==> (⊆)) assert_lift.
+Instance: Proper ((⊆@{δ}) ==> (⊆@{δ})) assert_lift.
 Proof. solve_assert. Qed.
-Instance: Proper ((≡) ==> (≡)) assert_lift.
+Instance: Proper ((≡@{δ}) ==> (≡@{δ})) assert_lift.
 Proof. solve_assert. Qed.
 
 Instance assert_lift_stack_indep: StackIndep P → StackIndep (P↑).
 Proof. solve_assert. Qed.
-Lemma stack_indep_lift `{StackIndep P} : (P↑)%A ≡ P.
+Lemma stack_indep_lift P `{StackIndep P} δ : (P↑)%A ≡@{δ} P.
 Proof. solve_assert. Qed.
 
 (** The assertion [assert_forall2 P xs ys] asserts that [P x y] holds for each
@@ -1013,8 +1153,9 @@ Definition assert_forall2 `(P : A → B → assert) : list A → list B → asse
   end%A.
 
 (** An alternative semantic formulation of the above assertion. *)
-Lemma assert_forall2_correct `(P : A → B → assert) xs ys ρ m :
-  assert_forall2 P xs ys ρ m ↔ Forall2 (λ x y, P x y ρ m) xs ys.
+Lemma assert_forall2_correct `(P : A → B → assert) δ ρ m xs ys :
+  assert_holds δ (assert_forall2 P xs ys) ρ m ↔
+    Forall2 (λ x y, assert_holds δ (P x y) ρ m) xs ys.
 Proof.
   split.
   * revert ys. induction xs; intros [|??]; solve_assert.
@@ -1025,10 +1166,10 @@ Qed.
 { var 0 ↦ - * Q↑ }] implies [{P} s {Q}]. We prove that this pre and
 postcondition is correct with respect to allocation of a local variable when
 entering a block and freeing a local variable when leaving a block. *)
-Lemma assert_alloc (P : assert) b v γ ρ m :
+Lemma assert_alloc (P : assert) δ ρ m b v γ :
   is_free m b →
-  P ρ m →
-  (var 0 ↦{γ} - ★ P↑)%A (b :: ρ) (mem_alloc b v γ m).
+  assert_holds δ P ρ m →
+  assert_holds δ (var 0 ↦{γ} - ★ P↑)%A (b :: ρ) (mem_alloc b v γ m).
 Proof.
   intros ??. eexists {[(b,v,γ)]}, m. split_ands.
   * by rewrite mem_alloc_singleton_l.
@@ -1037,10 +1178,10 @@ Proof.
   * done.
 Qed.
 
-Lemma assert_free (P : assert) b γ ρ m :
+Lemma assert_free (P : assert) δ ρ m b γ :
   ¬perm_fragment γ →
-  (var 0 ↦{γ} - ★ P↑)%A (b :: ρ) m →
-  P ρ (delete b m) ∧ mem_perm b m = Some γ.
+  assert_holds δ (var 0 ↦{γ} - ★ P↑)%A (b :: ρ) m →
+  assert_holds δ P ρ (delete b m) ∧ mem_perm b m = Some γ.
 Proof.
   intros ? (m1 & m2 &?&?& (a&v&?&?) &?); simplify_equality. split.
   * rewrite mem_delete_union, mem_delete_singleton, (left_id ∅ _),
@@ -1053,52 +1194,56 @@ Qed.
 (** We prove some properties related to allocation of local variables when
 calling a function, and to freeing these when returning from the function
 call. *)
-Lemma assert_alloc_params (P : assert) ρ m1 γ bs vs m2 :
+Lemma assert_alloc_params (P : assert) δ ρ m1 γ bs vs m2 :
   StackIndep P →
   alloc_params γ m1 bs vs m2 →
-  P ρ m1 →
-  (Π imap (λ i v, var i ↦{γ} val v) vs ★ P)%A (bs ++ ρ) m2.
+  assert_holds δ P ρ m1 →
+  assert_holds δ (Π imap (λ i v, var i ↦{γ} val v) vs ★ P)%A (bs ++ ρ) m2.
 Proof.
   intros ? Halloc ?. cut (∀ bs',
-    (Π imap_go (λ i v, var i ↦{γ} val v) (length bs') vs ★ P)%A
+    assert_holds δ (Π imap_go (λ i v, var i ↦{γ} val v) (length bs') vs ★ P)%A
       (bs' ++ bs ++ ρ) m2).
   { intros aux. by apply (aux []). }
   induction Halloc as [| b bs v vs m2 ?? IH ]; intros bs'; simpl.
-  * rewrite (left_id emp (★))%A. by apply (stack_indep ρ).
+  * rewrite (left_id emp (★))%A. by apply (stack_indep δ ρ).
   * rewrite <-(associative (★))%A. eexists {[(b,v,γ)]}, m2. split_ands.
     + by rewrite mem_alloc_singleton_l.
     + by apply mem_disjoint_singleton_l.
-    + exists b v. split_ands; trivial. simpl. by rewrite list_lookup_middle.
+    + exists b v. split_ands; trivial.
+      simpl. by rewrite list_lookup_middle.
     + specialize (IH (bs' ++ [b])). rewrite app_length in IH. simpl in IH.
       by rewrite NPeano.Nat.add_1_r, <-(associative (++)) in IH.
 Qed.
 
-Lemma assert_alloc_params_alt (P : assert) ρ m γ bs vs :
+Lemma assert_alloc_params_alt (P : assert) δ ρ m γ bs vs :
   StackIndep P →
   same_length bs vs →
   is_free_list m bs →
-  P ρ m →
-  (Π imap (λ i v, var i ↦{γ} val v) vs ★ P)%A (bs ++ ρ)
+  assert_holds δ P ρ m →
+  assert_holds δ (Π imap (λ i v, var i ↦{γ} val v) vs ★ P)%A (bs ++ ρ)
     (mem_alloc_list γ (zip bs vs) m).
 Proof. eauto using assert_alloc_params, alloc_params_alloc_list_2. Qed.
 
-Lemma assert_free_params (P : assert) ρ m γ bs (vs : list value) :
+Lemma assert_free_params (P : assert) δ ρ m γ bs (vs : list value) :
   StackIndep P →
   ¬perm_fragment γ →
   same_length bs vs →
   NoDup bs → (* admissible *)
-  (Π imap (λ i _, var i ↦{γ} -) vs ★ P)%A (bs ++ ρ) m →
-  P ρ (delete_list bs m) ∧ Forall (λ b, mem_perm b m = Some γ) bs.
+  assert_holds δ (Π imap (λ i _, var i ↦{γ} -) vs ★ P)%A (bs ++ ρ) m →
+  assert_holds δ P ρ (delete_list bs m) ∧
+    Forall (λ b, mem_perm b m = Some γ) bs.
 Proof.
   intros ?? Hlength. revert m. cut (∀ bs' m,
     NoDup bs →
-    (Π imap_go (λ i _, var i ↦{γ} -) (length bs') vs ★ P)%A (bs'++bs++ρ) m →
-    P ρ (delete_list bs m) ∧ Forall (λ b, mem_perm b m = Some γ) bs).
+    assert_holds δ (Π imap_go (λ i _, var i ↦{γ} -) (length bs') vs ★ P)%A
+      (bs' ++ bs ++ ρ) m →
+    assert_holds δ P ρ (delete_list bs m) ∧
+      Forall (λ b, mem_perm b m = Some γ) bs).
   { intros aux. by apply (aux []). }
   induction Hlength as [|b v bs vs ? IH];
     intros bs' m; simpl; inversion_clear 1.
   * rewrite (left_id emp (★))%A. split; [|done].
-    by apply (stack_indep (bs' ++ ρ)).
+    by apply (stack_indep δ (bs' ++ ρ)).
   * rewrite <-(associative (★))%A.
     intros (m1 & m2 & ? & ? & (b' & v' & Heval & ?) & ?).
     simplify_equality. simpl in Heval.
