expression_eval.v
@@ -1,166 +1,237 @@
 (* Copyright (c) 2012-2013, Robbert Krebbers. *)
 (* This file is distributed under the terms of the BSD license. *)
 (** This file defines a denotational semantics [⟦ _ ⟧] for pure expressions as
-an expression evaluator. *)
-Require Export expressions abstract_memory.
+an expression evaluator. It is parametrized by a map of function names to
+denotations. We use this to enable convenient reasoning about pure functions
+in our axiomatic semantics. *)
+Require Export fin_map_dom expressions abstract_memory.
 
+(** The type [purefun] represents denotations of pure functions. *)
+Definition purefun := list value → option value.
+Notation purefuns := (funmap purefun).
+
+(** * Definition of the semantics *)
 Reserved Notation "⟦ e ⟧" (format "⟦  e  ⟧").
-
 Section expression_eval.
 Context `{Permissions P}.
 
-(** * Definition of the semantics *)
-Fixpoint expr_eval (e : expr) (ρ : stack) (m : amem P) : option value :=
+Fixpoint expr_eval (e : expr)
+    (δ : purefuns) (ρ : stack) (m : amem P) : option value :=
   match e with
   | var x =>
      b ← ρ !! x;
      Some (ptr b)%V
   | load e =>
-     v ← ⟦ e ⟧ ρ m;
+     v ← ⟦ e ⟧ δ ρ m;
      a ← maybe_ptr v;
      m !! a
-  | val@{_} v => Some v
+  | val@{Ω} v =>
+     guard (Ω = ∅); Some v
   | ⊙{op} e =>
-     v ← ⟦ e ⟧ ρ m;
+     v ← ⟦ e ⟧ δ ρ m;
      eval_unop op v
   | el ⊙{op} er =>
-     vl ← ⟦ el ⟧ ρ m;
-     vr ← ⟦ er ⟧ ρ m;
+     vl ← ⟦ el ⟧ δ ρ m;
+     vr ← ⟦ er ⟧ δ ρ m;
      eval_binop op vl vr
+  | call f @ es =>
+     F ← δ !! f;
+     vs ← mapM (λ e, ⟦ e ⟧ δ ρ m) es;
+     F vs
+  | (IF e then el else er) =>
+     v ← ⟦ e ⟧ δ ρ m;
+     vl ← ⟦ el ⟧ δ ρ m;
+     vr ← ⟦ er ⟧ δ ρ m;
+     Some $ if value_true_false_dec v then vl else vr
   | _ => None
   end%E
 where "⟦ e ⟧" := (expr_eval e) : C_scope.
 
 (** * Theorems *)
+Lemma expr_eval_val δ ρ m v : ⟦ val v ⟧ δ ρ m = Some v.
+Proof. done. Qed.
+
+Lemma mapM_expr_eval_val δ ρ m Ωs vs :
+  same_length Ωs vs →
+  ⋃ Ωs = ∅ →
+  mapM (λ e, ⟦ e ⟧ δ ρ m) (zip_with EVal Ωs vs) = Some vs.
+Proof.
+  rewrite empty_union_list_L.
+  induction 1; intros; decompose_Forall; simplify_option_equality; auto.
+Qed.
+Lemma Forall2_expr_eval_val_inv δ ρ m Ωs vs ws:
+  same_length Ωs vs →
+  Forall2 (λ e v, ⟦ e ⟧ δ ρ m = Some v) (zip_with EVal Ωs vs) ws →
+  vs = ws.
+Proof.
+  intros HΩvs. revert ws.
+  induction HΩvs; simpl; intros; decompose_Forall;
+    simplify_option_equality; f_equal; eauto.
+Qed.
+
 (** We prove that we only give a semantics to pure expressions. The converse
 of this property is not true, as pure expressions may still exhibit undefined
 behavior. *)
-Lemma expr_eval_is_pure ρ m e v :
-  ⟦ e ⟧ ρ m = Some v → is_pure e.
+Lemma expr_eval_is_pure δ ρ m e v :
+  ⟦ e ⟧ δ ρ m = Some v → is_pure (dom _ δ) e.
 Proof.
-  revert v.
-  induction e; intros; simplify_option_equality; constructor; eauto.
+  revert v. induction e using expr_ind_alt; intros;
+    simplify_option_equality;
+    try destruct (value_true_false_dec _);
+    constructor; eauto.
+  * apply elem_of_dom; eauto.
+  * decompose_Forall; eauto.
 Qed.
 
-(** Evaluation of expressions is preserved under extensions of the memory. *)
-Lemma expr_eval_weaken_mem ρ m1 m2 e v :
-  ⟦ e ⟧ ρ m1 = Some v →
+(** Evaluation of pure expressions is preserved under extensions of the
+memory. *)
+Lemma expr_eval_weaken_mem δ ρ m1 m2 e v :
+  ⟦ e ⟧ δ ρ m1 = Some v →
   m1 ⊆ m2 →
-  ⟦ e ⟧ ρ m2 = Some v.
+  ⟦ e ⟧ δ ρ m2 = Some v.
 Proof.
-  revert v. induction e; intros; simplify_option_equality; eauto.
-  eapply mem_lookup_weaken; eauto.
+  revert v. induction e using expr_ind_alt; intros;
+    simplify_option_equality; eauto.
+  * erewrite mapM_Some_2; [by eauto|]. decompose_Forall; auto.
+  * eapply mem_lookup_weaken; eauto.
 Qed.
 
-Lemma expr_eval_weaken_inv ρ m1 m2 e v1 v2 :
-  ⟦ e ⟧ ρ m1 = Some v1 →
+Lemma expr_eval_weaken_inv δ ρ m1 m2 e v1 v2 :
+  ⟦ e ⟧ δ ρ m1 = Some v1 →
   m1 ⊆ m2 →
-  ⟦ e ⟧ ρ m2 = Some v2 →
+  ⟦ e ⟧ δ ρ m2 = Some v2 →
   v1 = v2.
 Proof.
   intros ? Hm1 Hm2.
-  erewrite (expr_eval_weaken_mem _ m1 m2) in Hm2 by eauto.
+  erewrite (expr_eval_weaken_mem _ _ m1 m2) in Hm2 by eauto.
   congruence.
 Qed.
 
-Lemma Forall_expr_eval_weaken_inv es ρ m1 m2 vs1 vs2 :
-  Forall2 (λ e v, ⟦ e ⟧ ρ m1 = Some v) es vs1 →
+Lemma Forall_expr_eval_weaken_inv δ ρ m1 m2 es vs1 vs2 :
+  Forall2 (λ e v, ⟦ e ⟧ δ ρ m1 = Some v) es vs1 →
   m1 ⊆ m2 →
-  Forall2 (λ e v, ⟦ e ⟧ ρ m2 = Some v) es vs2 →
+  Forall2 (λ e v, ⟦ e ⟧ δ ρ m2 = Some v) es vs2 →
   vs1 = vs2.
 Proof.
   intros ? Hm1 ?.
-  apply (Forall2_unique (λ e v, ⟦ e ⟧ ρ m2 = Some v) es).
-  * apply Forall2_impl with (λ e v, ⟦ e ⟧ ρ m1 = Some v);
+  apply (Forall2_unique (λ e v, ⟦ e ⟧ δ ρ m2 = Some v) es).
+  * apply Forall2_impl with (λ e v, ⟦ e ⟧ δ ρ m1 = Some v);
       eauto using expr_eval_weaken_mem.
   * done.
   * congruence.
 Qed.
 
-(** Evaluation of expressions is preserved under unlocking. *)
-Lemma expr_eval_unlock Ω ρ m e v :
-  ⟦ e ⟧ ρ m = Some v →
-  ⟦ e ⟧ ρ (mem_unlock Ω m) = Some v.
+(** Evaluation of pure expressions is preserved under unlocking. *)
+Lemma expr_eval_unlock δ Ω ρ m e v :
+  ⟦ e ⟧ δ ρ m = Some v →
+  ⟦ e ⟧ δ ρ (mem_unlock Ω m) = Some v.
 Proof.
-  revert v. induction e; intros; simplify_option_equality; eauto.
-  eapply mem_lookup_unlock; eauto.
+  revert v. induction e using expr_ind_alt; intros;
+    simplify_option_equality; eauto.
+  * erewrite mapM_Some_2; [by eauto |]. decompose_Forall; auto.
+  * eapply mem_lookup_unlock; eauto.
 Qed.
 
-(** Evaluation of expressions is preserved under extensions of the stack. *)
-Lemma expr_eval_weaken_stack ρ ρ' m e v :
-  ⟦ e ⟧ ρ m = Some v →
-  ⟦ e ⟧ (ρ ++ ρ') m = Some v.
+(** Evaluation of pure expressions is preserved under extensions of the
+stack. *)
+Lemma expr_eval_weaken_stack δ ρ ρ' m e v :
+  ⟦ e ⟧ δ ρ m = Some v →
+  ⟦ e ⟧ δ (ρ ++ ρ') m = Some v.
 Proof.
-  revert v. induction e; intros; simplify_option_equality; intuition.
-  rewrite lookup_app_l.
-  * by simplify_option_equality.
-  * eauto using lookup_lt_length_alt.
+  revert v. induction e using expr_ind_alt;
+    intros; simplify_option_equality; intuition.
+  * rewrite lookup_app_l.
+    + by simplify_option_equality.
+    + eauto using lookup_lt_length_alt.
+  * erewrite mapM_Some_2; [by eauto |]. decompose_Forall; auto.
 Qed.
 
 (** Pure expressions without variables do not refer to the stack, so their
 semantics is preserved under changes to the stack. *)
-Lemma expr_var_free_stack_indep ρ1 ρ2 m e :
-  expr_vars e ≡ ∅ →
-  ⟦ e ⟧ ρ1 m = ⟦ e ⟧ ρ2 m.
+Lemma expr_var_free_stack_indep δ ρ1 ρ2 m e :
+  vars e ≡ ∅ →
+  ⟦ e ⟧ δ ρ1 m = ⟦ e ⟧ δ ρ2 m.
 Proof.
-  induction e; simpl; intro; decompose_empty; repeat
+  induction e using expr_ind_alt; simpl; intro; decompose_empty; repeat
     match goal with
-    | H : expr_vars _ ≡ ∅ → ⟦ _ ⟧ _ _ = _ |- _ => rewrite H
+    | H : vars _ ≡ ∅ → ⟦ _ ⟧ _ _ _ = _ |- _ => rewrite H
+    | H : ⋃ _ ≡ ∅ |- _ => rewrite empty_union_list in H
     | _ => done
-    | |- mbind (M:=option) _ ?o = mbind (M:=option) _ ?o =>
-       destruct o; simpl
-    | _ => destruct (value_true_false_dec _)
     end.
+  apply option_bind_ext_fun. intros.
+  f_equal. apply Forall_mapM_ext. decompose_Forall; auto.
 Qed.
 
-(** Pure expressions without loads do not refer to the memory, so their
+(** Pure expressions that are load free do not refer to the memory, so their
 semantics is preserved under changes to the memory. *)
-Lemma expr_load_free_mem_indep ρ m1 m2 e :
+Lemma expr_load_free_mem_indep δ ρ m1 m2 e :
   load_free e →
-  ⟦ e ⟧ ρ m1 = ⟦ e ⟧ ρ m2.
+  ⟦ e ⟧ δ ρ m1 = ⟦ e ⟧ δ ρ m2.
 Proof.
-  induction 1; simpl; repeat
+  induction 1 using load_free_ind_alt; simpl; repeat
     match goal with
-    | H : ⟦ _ ⟧ _ _ = _ |- _ => rewrite H
+    | H : ⟦ _ ⟧ _ _ _ = _ |- _ => rewrite H
     | _ => done
-    | |- mbind (M:=option) _ ?o = mbind (M:=option) _ ?o =>
-       destruct o; simpl
-    | _ => destruct (value_true_false_dec _)
     end.
+  apply option_bind_ext_fun. intros. f_equal. by apply Forall_mapM_ext.
+Qed.
+
+(** Only the denotations of functions that actually appear in an expression
+are relevant. *)
+Lemma expr_eval_fun_irrel δ1 δ2 ρ m e :
+  (∀ f, f ∈ funs e → δ1 !! f = δ2 !! f) →
+  ⟦ e ⟧ δ1 ρ m = ⟦ e ⟧ δ2 ρ m.
+Proof.
+  assert (∀ f es i e', 
+    es !! i = Some e' →
+    f ∈ funs e' → f ∈ ⋃ (funs <$> es)).
+  { intros ???? Hi Hf. apply elem_of_union_list.
+    exists (funs e'). split; eauto.
+    eapply elem_of_list_fmap_1, elem_of_list_lookup_2; eauto. }
+  intros Hfs.
+  induction e using expr_ind_alt; simpl in *; try done;
+    repeat (apply option_bind_ext; intros); eauto;
+    try solve_elem_of.
+  apply Forall_mapM_ext. decompose_Forall. esolve_elem_of.
 Qed.
 
 (** Lifting DeBruijn indexes distributes over expression evaluation. *)
-Lemma expr_eval_lift ρ e m :
-  ⟦ e↑ ⟧ ρ m = ⟦ e ⟧ (tail ρ) m.
+Lemma expr_eval_lift δ ρ m e :
+  ⟦ e↑ ⟧ δ ρ m = ⟦ e ⟧ δ (tail ρ) m.
 Proof.
-  induction e; intros; simpl; repeat
+  induction e using expr_ind_alt; intros; simpl; repeat
     match goal with
-    | H : ⟦ _↑ ⟧ _ _ = _ |- _ => rewrite H
-    | |- _ ← ?o; ⟦ if _ then _ else _ ⟧ _ _ = _ =>
-      destruct o; simpl; try destruct (value_true_false_dec _)
+    | H : ⟦ _↑ ⟧ _ _ _ = _ |- _ => rewrite H
     end; auto.
-  by rewrite <-lookup_tail.
+  * by rewrite <-lookup_tail.
+  * destruct (δ !! _); simpl; [|done].
+    f_equal. apply Forall2_mapM_ext. by decompose_Forall.
 Qed.
 
-(** If an expression has a semantics, then each sub-expression has a semantics
-as well. *)
-Lemma expr_eval_subst_inv (E : ectx) e ρ m v :
-  ⟦ subst E e ⟧ ρ m = Some v →
-  ∃ v', ⟦ e ⟧ ρ m = Some v' ∧ ⟦ subst E (val v')%E ⟧ ρ m = Some v.
+(** If an expression has a semantics, then each sub-expression of that
+expression has a semantics too. *)
+Lemma expr_eval_subst_inv δ ρ m (E : ectx) e v :
+  ⟦ subst E e ⟧ δ ρ m = Some v →
+  ∃ v', ⟦ e ⟧ δ ρ m = Some v' ∧ ⟦ subst E (val v')%E ⟧ δ ρ m = Some v.
 Proof.
   revert v. induction E as [|E' E IH] using rev_ind;
-    simpl; intros v; [by eauto |].
+    simpl; intros v; [eauto |].
   setoid_rewrite subst_snoc.
   intros; destruct E'; simplify_option_equality;
-    naive_solver (by eauto || by simplify_option_equality).
+    try solve [edestruct IH as (?&?&?); eauto with simplify_option_equality].
+  decompose_Forall. edestruct IH as (?&?&?); eauto.
+  eexists; split_ands; eauto.
+  erewrite mapM_Some_2; [by eauto |]. decompose_Forall; eauto.
 Qed.
 
-Lemma subst_preserves_expr_eval (E : ectx) e1 e2 ρ m :
-  ⟦ e1 ⟧ ρ m = ⟦ e2 ⟧ ρ m →
-  ⟦ subst E e1 ⟧ ρ m = ⟦ subst E e2 ⟧ ρ m.
+Lemma subst_preserves_expr_eval δ ρ m (E : ectx) e1 e2 :
+  ⟦ e1 ⟧ δ ρ m = ⟦ e2 ⟧ δ ρ m →
+  ⟦ subst E e1 ⟧ δ ρ m = ⟦ subst E e2 ⟧ δ ρ m.
 Proof.
   intros. induction E as [|E' ? IH] using rev_ind; [done |].
   destruct E'; rewrite ?subst_snoc; simpl; rewrite ?IH; auto.
+  destruct (δ !! _); simpl; [|done].
+  f_equal. apply Forall2_mapM_ext. by decompose_Forall.
 Qed.
 End expression_eval.
 
@@ -179,9 +250,9 @@ Tactic Notation "simplify_expr_equality" "by" tactic3(tac) := repeat
     destruct (value_true_false_dec v)
   | |- context [ value_true_false_dec ?v ] =>
     destruct (value_true_false_dec v)
-  | H1 : ⟦ ?e ⟧ ?ρ ?m1 = Some ?v1, H2 : ⟦ ?e ⟧ ?ρ ?m2 = Some ?v2 |- _ =>
+  | H1: ⟦ ?e ⟧ ?δ ?ρ ?m1 = Some ?v1, H2: ⟦ ?e ⟧ ?δ ?ρ ?m2 = Some ?v2 |- _ =>
     let H3 := fresh in
-    feed pose proof (expr_eval_weaken_inv e ρ m1 m2 v1 v2) as H3;
+    feed pose proof (expr_eval_weaken_inv ρ m1 m2 e v1 v2) as H3;
       [done | by tac | done | ];
     clear H2; symmetry in H3
   end.
