expression_eval_correct.v
@@ -4,55 +4,77 @@
 pure expressions and the small step operational semantics. *)
 Require Export smallstep expression_eval.
 
-Lemma ehstep_expr_eval_inv ρ m v e1 m1 e2 m2 :
+Lemma ehstep_expr_eval_inv δ ρ m v e1 m1 e2 m2 :
   ρ ⊢ₕ e1, m1 ⇒ e2, m2 →
-  ⟦ e1 ⟧ ρ m = Some v →
+  ⟦ e1 ⟧ δ ρ m = Some v →
   m ⊆ m1 →
-  m2 = m1 ∧ ⟦ e2 ⟧ ρ m = Some v.
-Proof. by destruct 1; intros; simplify_expr_equality. Qed.
-
-Lemma ehstep_expr_eval ρ e1 m v :
-  ⟦ e1 ⟧ ρ m = Some v →
-  is_redex e1 →
-  ∃ e2, ρ ⊢ₕ e1, m ⇒ e2, m ∧ ⟦ e2 ⟧ ρ m = Some v.
+  m2 = m1 ∧ ⟦ e2 ⟧ δ ρ m = Some v.
 Proof.
-  destruct 2;
+  by destruct 1; intros; try solve [simplify_expr_equality;
+    rewrite ?mem_unlock_empty_locks; eauto].
+Qed.
+
+Lemma ehstep_expr_eval δ ρ e1 m v :
+  ⟦ e1 ⟧ δ ρ m = Some v →
+  is_redex e1 →
+  (∃ e2, ρ ⊢ₕ e1, m ⇒ e2, m ∧ ⟦ e2 ⟧ δ ρ m = Some v) ∨
+  (∃ f F Ωs vs,
+    e1 = (call f @ zip_with EVal Ωs vs)%E ∧
+    same_length Ωs vs ∧
+    δ !! f = Some F ∧
+    F vs = Some v).
+Proof.
+  destruct 2; intros;
     repeat match goal with
     | H : is_value _ |- _ => inversion H; subst; clear H
-    end;
-    intros; simplify_expr_equality; eexists; by (split; [do_ehstep |]).
+    | H : Forall is_value _ |- _ =>
+      apply Forall_is_value_alt in H; destruct H as (?&?&?&?)
+    | H : Forall2 (λ e v, ⟦ e ⟧ _ _ _ = Some v) _ _ |- _ =>
+      apply Forall2_expr_eval_val_inv in H; [| done]
+    | _ => progress simplify_expr_equality
+    end; try naive_solver (eauto; do_ehstep).
 Qed.
 
-Lemma ehstep_expr_eval_subst ρ (E : ectx) e1 m v :
-  ⟦ subst E e1 ⟧ ρ m = Some v →
+Lemma ehstep_expr_eval_subst δ ρ m (E : ectx) e1 v :
+  ⟦ subst E e1 ⟧ δ ρ m = Some v →
   is_redex e1 →
-  ∃ e2, ρ ⊢ₕ e1, m ⇒ e2, m ∧ ⟦ subst E e2 ⟧ ρ m = Some v.
+  (∃ e2, ρ ⊢ₕ e1, m ⇒ e2, m ∧ ⟦ subst E e2 ⟧ δ ρ m = Some v) ∨
+  (∃ f F Ωs vs w,
+    e1 = (call f @ zip_with EVal Ωs vs)%E ∧
+    same_length Ωs vs ∧
+    δ !! f = Some F ∧
+    F vs = Some w ∧
+    ⟦ subst E (val w)%E ⟧ δ ρ m = Some v).
 Proof.
   intros Heval ?.
-  destruct (expr_eval_subst_inv _ _ _ _ _ Heval) as [v' [Heval' ?]].
-  destruct (ehstep_expr_eval _ _ _ _ Heval') as [e2 [??]]; trivial.
-  exists e2. split; [done |].
-  rewrite (subst_preserves_expr_eval _ _ e1); congruence.
+  destruct (expr_eval_subst_inv _ _ _ _ _ _ Heval) as [v' [Heval' ?]].
+  destruct (ehstep_expr_eval _ _ _ _ _ Heval')
+    as [(e2&?&?)|(f&F&Ωs&vs&?&?&?&?)]; trivial.
+  * left. exists e2. split; [done |].
+    rewrite (subst_preserves_expr_eval _ _ _ _ _ e1); congruence.
+  * right. exists f F Ωs vs. exists v'. eauto.
 Qed.
 
-Lemma ehsafe_expr_eval_subst ρ (E : ectx) e m v :
-  ⟦ subst E e ⟧ ρ m = Some v →
+Lemma ehsafe_expr_eval_subst δ ρ m (E : ectx) e v :
+  ⟦ subst E e ⟧ δ ρ m = Some v →
   is_redex e →
   ρ ⊢ₕ safe e, m.
 Proof.
   intros Heval ?.
-  destruct (ehstep_expr_eval_subst _ _ _ _ _ Heval) as [? [??]];
-    eauto using ehsafe_step.
+  destruct (ehstep_expr_eval_subst _ _ _ _ _ _ Heval)
+    as [(e2&?&?)|(f&F&vs&?&?&?&?&?)]; trivial; subst.
+  * eauto using ehsafe_step.
+  * by constructor.
 Qed.
 
-Lemma cred_expr_eval δ e k m v :
-  ⟦ e ⟧ (get_stack k) m = Some v →
+Lemma cred_expr_eval δp δ e k m v :
+  ⟦ e ⟧ δp (get_stack k) m = Some v →
   ¬is_value e →
   red (cstep_in_ctx δ k) (State k (Expr e) m).
 Proof.
   intros Heval He.
   destruct (is_value_is_redex _ He) as [E' [e' [??]]]; subst.
-  destruct (expr_eval_subst_inv _ _ _ _ _ Heval) as [v' [??]].
-  destruct (ehstep_expr_eval_subst _ _ _ _ _ Heval) as [? [??]]; trivial.
-  solve_cred.
+  destruct (expr_eval_subst_inv _ _ _ _ _ _ Heval) as [v' [??]].
+  destruct (ehstep_expr_eval_subst _ _ _ _ _ _ Heval)
+    as [(e2&?&?)|(f&F&vs&?&?&?&?&?)]; trivial; subst; solve_cred.
 Qed.
